add proof technique for prepost

theories/imp.v
@@ -89,6 +89,9 @@ Proof.
   all: auto.
 Qed.
 
+Global Instance val_inj : Inj (=) (=) Val.
+Proof. move => ?? []. done. Qed.
+
 Definition to_val (e : expr) : option val :=
   match e with
   | Val v => Some v
@@ -638,6 +641,24 @@ Proof.
 Qed.
 Global Hint Resolve imp_step_ReturnExt_s : tstep.
 
+Lemma imp_step_Call_i fns h e K f vs `{!ImpExprFill e K (imp.Call f (Val <$> vs))}:
+  TStepI imp_module (Imp e h fns) (λ G,
+    (∀ fn, fns !! f = Some fn → G true None (λ G', length vs = length fn.(fd_args) ∧
+         G' (Imp (expr_fill K (subst_l fn.(fd_args) vs fn.(fd_body))) h fns))) ∧
+    (fns !! f = None → G true (Some (Outgoing, EICall f vs h)) (λ G',
+           G' (Imp (expr_fill K (Waiting true)) h fns)))).
+Proof.
+  destruct ImpExprFill0; subst.
+  constructor => ? HG. apply steps_impl_step_end => ?? /prim_step_inv_head[| |?[??]]. {
+    apply sub_redexes_are_values_item; case; try naive_solver.
+    move => /= ??? e' [_ Heq]. by apply: list_expr_val_inv.
+  } { done. } subst.
+  invert_all head_step.
+  - naive_solver.
+  - naive_solver.
+Qed.
+Global Hint Resolve imp_step_Call_i : tstep.
+
 Lemma imp_step_Call_s fns h e K f vs `{!ImpExprFill e K (imp.Call f (Val <$> vs))}:
   TStepS imp_module (Imp e h fns) (λ G,
     (∃ fn, fns !! f = Some fn ∧ G None (λ G', length vs = length fn.(fd_args) → G'
@@ -852,6 +873,136 @@ Proof.
 Qed.
 Global Hint Resolve imp_step_If_s | 10 : tstep.
 
+(** * proof technique for prepost *)
+Inductive imp_prepost_proof_stack {S} (n : trace_index) (fnsi fnss : gmap string fndef) i o R :
+  bool → S → list expr_ectx → list expr_ectx → Prop :=
+| IPSNil s :
+  imp_prepost_proof_stack n fnsi fnss i o R false s [] []
+| IPSStep b Ki Ki' Ks Ks' s0 s1:
+  imp_prepost_proof_stack n fnsi fnss i o R b s0 Ki Ks →
+  (∀ hi vi s2,
+      R true s1 s2 →
+      pp_to_all (i (Incoming, EIReturn vi hi) s2) (λ '(e', s3),
+      ∃ vs hs, e' = (Incoming, EIReturn vs hs) ∧
+      Imp (expr_fill (Ki' ++ Ki) (Val vi)) hi fnsi
+        ⪯{imp_module, mod_prepost (S:=S) i o imp_module, n, true}
+        (SMProg, Imp (expr_fill (Ks' ++ Ks) (Val vs)) hs fnss, (PPInside, s3)))) →
+  imp_prepost_proof_stack n fnsi fnss i o R true s1 (Ki' ++ Ki) (Ks' ++ Ks)
+.
+
+Lemma imp_prepost_proof_stack_mono S n n' fns1 fns2 i o R s b Ki Ks:
+  imp_prepost_proof_stack n fns1 fns2 i o R b s Ki Ks →
+  n' ⊆ n →
+  imp_prepost_proof_stack (S:=S) n' fns1 fns2 i o R b s Ki Ks.
+Proof.
+  move => Hs. elim: Hs n'; [by econs|].
+  move => *. econs; [naive_solver|] => *.
+  apply: pp_to_all_mono; [naive_solver|]. move => [??] ?. destruct_all?; subst. split!.
+  by apply: tsim_mono.
+Qed.
+
+Lemma imp_prepost_proof_stack_mono_R S n fns1 fns2 i o R s s' b Ki Ks `{!Transitive (R true)}:
+  imp_prepost_proof_stack n fns1 fns2 i o R b s Ki Ks →
+  R true s s' →
+  imp_prepost_proof_stack (S:=S) n fns1 fns2 i o R b s' Ki Ks.
+Proof.
+  move => Hs. elim: Hs s'; [by econs|].
+  move => ????????? Hcont ??. econs; [naive_solver|] => *.
+  apply: pp_to_all_mono. { apply Hcont. by etrans. } done.
+Qed.
+
+Lemma imp_prepost_proof {S} R `{!∀ b, PreOrder (R b)} i o fns1 fns2 s0:
+  (* R true: public transition relation, R false: private transition relation *)
+  (∀ s s', R true s s' → R false s s') →
+  (∀ n K1 K2 f fn1 vs1 h1 s1,
+      R false s0 s1 →
+      fns1 !! f = Some fn1 →
+      pp_to_all (i (Incoming, EICall f vs1 h1) s1) (λ '(e', s2),
+      ∃ vs2 h2 fn2, e' = (Incoming, EICall f vs2 h2) ∧ fns2 !! f = Some fn2 ∧ (
+        length vs2 = length (fd_args fn2) →
+          length vs1 = length (fd_args fn1) ∧ (
+      (* Call *)
+      (∀ n' f K1' K2' es1 es2 vs1' vs2' h1' h2' b s3,
+         n' ⊆ n →
+         fns1 !! f = None →
+         fns2 !! f = None →
+         Forall2 (λ e v, e = Val v) es1 vs1' →
+         Forall2 (λ e v, e = Val v) es2 vs2' →
+         pp_to_ex (o (Outgoing, EICall f vs2' h2') s3) (λ '(e''', s4),
+            e''' = (Outgoing, EICall f vs1' h1') ∧ R false s1 s4 ∧
+           ∀ v1'' h1'' s5, R true s4 s5 → pp_to_all (i (Incoming, EIReturn v1'' h1'') s5) (λ '(e''''', s6),
+            ∃ v2'' h2'', e''''' = (Incoming, EIReturn v2'' h2'') ∧
+          Imp (expr_fill K1 (expr_fill K1' (Val v1''))) h1'' fns1
+              ⪯{imp_module, mod_prepost i o imp_module, n', true}
+          (SMProg, Imp (expr_fill K2 (expr_fill K2' (Val v2''))) h2'' fns2, (PPInside, s6)))) →
+
+          Imp (expr_fill K1 (expr_fill K1' (Call f es1))) h1' fns1
+              ⪯{imp_module, mod_prepost i o imp_module, n', b}
+          (SMProg, Imp (expr_fill K2 (expr_fill K2' (Call f es2))) h2' fns2, (PPInside, s3))) →
+      (* Return *)
+      (∀ n' v1 v2 h1' h2' b s3,
+         n' ⊆ n →
+         pp_to_ex (o (Outgoing, EIReturn v2 h2') s3) (λ '(e''', s4),
+               e''' = (Outgoing, EIReturn v1 h1') ∧ R true s1 s4) →
+          Imp (expr_fill K1 (Val v1)) h1' fns1
+              ⪯{imp_module, mod_prepost i o imp_module, n', b}
+          (SMProg, Imp (expr_fill K2 (Val v2)) h2' fns2, (PPInside, s3))) →
+      Imp (expr_fill K1 (subst_l fn1.(fd_args) vs1 fn1.(fd_body))) h1 fns1
+          ⪯{imp_module, mod_prepost i o imp_module, n, false}
+          (SMProg, Imp (expr_fill K2 (subst_l fn2.(fd_args) vs2 fn2.(fd_body))) h2 fns2, (PPInside, s2)))))) →
+  trefines (MS imp_module (initial_imp_state fns1))
+           (MS (mod_prepost (S:=S) i o imp_module)
+               (SMFilter, initial_imp_state fns2, (PPOutside, s0))).
+Proof.
+  move => HR Hcall.
+  apply: tsim_implies_trefines => n.
+  unshelve apply: tsim_remember. { simpl. exact (λ n '(Imp ei hi fnsi) '(ips, Imp es hs fnss, (pp, s)),
+    ∃ Ki Ks b,
+      fnsi = fns1 ∧
+      fnss = fns2 ∧
+      ei = expr_fill Ki (Waiting b) ∧
+      es = expr_fill Ks (Waiting b) ∧
+      pp = PPOutside ∧
+      ips = SMFilter ∧
+      R false s0 s ∧
+      imp_prepost_proof_stack n fns1 fns2 i o R b s Ki Ks
+). }
+  { eexists [], []. split!. econs. } {
+    move => ? n' [ei hi fnsi] [[ips [es hs fnss]] [pp {}s]] /= Hsub ?. destruct_all?.
+    split!. 1, 2: done. by apply: imp_prepost_proof_stack_mono.
+  }
+  move => {}n _ /= Hloop [ei hi fnsi] [[ips [es hs fnss]] [pp {}s]] [Ki [Ks ?]].
+  destruct_all?; simplify_eq.
+  tstep_i. split => *.
+  - tstep_s. split!.
+    tstep_s. apply: pp_to_all_mono. { by eapply (Hcall n (ReturnExtCtx b :: Ki) (ReturnExtCtx b :: Ks)). }
+    move => -[??] [?[?[?[?[? Hcall']]]]]. simplify_eq/=.
+    tstep_s. left. split!. repeat case_bool_decide; try by tstep_s. 2: naive_solver.
+    have [//|? {}Hcall'] := Hcall'. apply: tsim_mono_b. apply: Hcall'.
+    + move => n' f K1' K2' es1 es2 vs1' vs2' ??????? Hall1 Hall2 ?.
+      have ?: es1 = Val <$> vs1'. { clear -Hall1. elim: Hall1; naive_solver. } subst.
+      have ?: es2 = Val <$> vs2'. { clear -Hall2. elim: Hall2; naive_solver. } subst.
+      tstep_i. split => *; simplify_eq. rewrite orb_true_r. tstep_s. right. split!.
+      tstep_s. apply: pp_to_ex_mono; [done|].
+      move => [??] /= [?[??]]. simplify_eq. split!.
+      apply: Hloop; [done|].
+      split!; [done..|by etrans|]. econs; [by apply: imp_prepost_proof_stack_mono|].
+      move => ????. apply: pp_to_all_mono; [naive_solver|].
+      move => [??] /= ?. destruct_all?. subst. split!.
+      rewrite !expr_fill_app /=. done.
+    + move => *. tstep_s. tstep_i. rewrite orb_true_r. tstep_s. apply: pp_to_ex_mono; [done|].
+      move => [??] [-> ?] /=. split!. apply: tsim_mono; [|done]. apply: Hloop; [done|].
+      split!. 1, 2: done.
+      { etrans; [done|]. by apply: HR. }
+      { by apply: imp_prepost_proof_stack_mono_R. }
+  - revert select (imp_prepost_proof_stack _ _ _ _ _ _ _ _ _ _) => Hs.
+    inversion Hs; clear Hs; simplify_eq/= => //.
+    tstep_s. split!.
+    tstep_s. apply: pp_to_all_mono; [naive_solver|].
+    move => [??] [?[?[? Hsim]]]; simplify_eq/=.
+    tstep_s. right. split!.
+Qed.
+
 (** * closing *)
 Definition imp_closed_val_to_Z (v : val) (z : Z) : Prop :=
   match v with
@@ -1022,14 +1173,14 @@ Proof.
       destruct el'; simplify_eq/=.
       inversion HK; clear HK; simplify_eq/=.
       * tstep_i. tstep_s. split!; [done..|] => /=. split!.
-        apply: Hloop. by split!.
+        apply: Hloop; [done|]. by split!.
       * tstep_s. split!.
         tstep_s. split!.
         rewrite !expr_fill_app. apply: IHm; [|done|]; [lia|]. split!. by apply static_expr_expr_fill.
     - destruct (to_val er') eqn:?; [ |apply: Hloop; naive_solver].
       destruct er'; simplify_eq/=.
       inversion HK; clear HK; simplify_eq/=.
-      * tstep_i. tstep_s. split!. apply: Hloop. by split!.
+      * tstep_i. tstep_s. split!. apply: Hloop; [done|]. by split!.
       * tstep_s. split!.
         tstep_s. split!.
         rewrite !expr_fill_app. apply: IHm; [|done|]; [lia|]. split!. by apply static_expr_expr_fill.
@@ -1146,85 +1297,85 @@ Proof.
       revert select (imp_link_prod_combine_ectx _ _ _ _ _ _ _ _) => HK.
       inversion HK; clear HK; simplify_eq/=.
       * tstep_i => *; destruct_all?; simplify_eq. tstep_s. split!.
-        apply Hloop. by split!.
+        apply: Hloop; [done|]. by split!.
       * tstep_i => *; destruct_all?; simplify_eq/=.
         tstep_i; split => *; simplify_eq.
-        apply Hloop. rewrite !expr_fill_app. split!; [done..|].
+        apply: Hloop; [done|]. rewrite !expr_fill_app. split!; [done..|].
         by apply static_expr_expr_fill.
     + tstep_both. apply: steps_impl_step_end => ?? /prim_step_inv[//|?[?[?[?[??]]]]] *.
       simplify_eq. revert select (Is_true (static_expr _ _)) => /static_expr_expr_fill/=[??]//.
       rewrite -expr_fill_app.
       invert_all head_step => //; destruct_all?; simplify_eq.
       * tstep_s => *. tend. split!; [done..|].
-        apply: Hloop. rewrite !expr_fill_app. split!; [done..| ].
+        apply: Hloop; [done|]. rewrite !expr_fill_app. split!; [done..| ].
         by apply static_expr_expr_fill.
       * tstep_s => *. tend. split!; [done..|].
-        apply: Hloop. rewrite !expr_fill_app. split!; [done..| ].
+        apply: Hloop; [done|]. rewrite !expr_fill_app. split!; [done..| ].
         by apply static_expr_expr_fill.
       * tstep_s => *. tend. split!; [done..|].
-        apply: Hloop. rewrite !expr_fill_app. split!; [done..| ].
+        apply: Hloop; [done|]. rewrite !expr_fill_app. split!; [done..| ].
         by apply static_expr_expr_fill.
       * tstep_s => *. split!; [done..|] => *. tend. split!; [done..|].
-        apply: Hloop. rewrite !expr_fill_app. split!; [done..| ].
+        apply: Hloop; [done|]. rewrite !expr_fill_app. split!; [done..| ].
         by apply static_expr_expr_fill.
       * tstep_s => *. tend. split!; [done..|].
-        apply: Hloop. rewrite !expr_fill_app. split!; [done..| ].
+        apply: Hloop; [done|]. rewrite !expr_fill_app. split!; [done..| ].
         by apply static_expr_expr_fill.
-      * tstep_s => b ?. subst. tend. split!. apply: Hloop. rewrite !expr_fill_app. split!; [done..| ].
+      * tstep_s => b ?. subst. tend. split!. apply: Hloop; [done|]. rewrite !expr_fill_app. split!; [done..| ].
         apply static_expr_expr_fill. split!. destruct b; naive_solver.
       * tstep_s => *. tend. split!; [done..|].
-        apply: Hloop. rewrite !expr_fill_app. split!; [done..| ].
+        apply: Hloop; [done|]. rewrite !expr_fill_app. split!; [done..| ].
         apply static_expr_expr_fill. split!. by apply static_expr_subst.
       * by tstep_s.
       * tstep_s. left. split!; [apply lookup_union_Some; naive_solver|] => ?. tend. split!; [done..|].
-        apply: Hloop. rewrite !expr_fill_app. split!; [done..|].
+        apply: Hloop; [done|]. rewrite !expr_fill_app. split!; [done..|].
         apply static_expr_expr_fill. split!. apply static_expr_subst_l; [|done].
         apply static_expr_mono. apply fd_static.
       * move => *. destruct_all?; simplify_eq/=. repeat case_bool_decide => //.
         -- have [??] : is_Some (fns2 !! f) by apply elem_of_dom.
            tstep_s. left. split!; [apply lookup_union_Some; naive_solver|] => ?. tend. split!.
            tstep_i. split => *; simplify_eq. case_bool_decide => //.
-           apply: Hloop. split!; [by econs|done..|].
+           apply: Hloop; [done|]. split!; [by econs|done..|].
            apply static_expr_subst_l; [|done]. apply static_expr_mono. apply fd_static.
         -- tstep_s. right. split!; [apply lookup_union_None;split!;by apply not_elem_of_dom| done|].
-           tend. split!. apply: Hloop. split!; [by econs|done..].
+           tend. split!. apply: Hloop; [done|]. split!; [by econs|done..].
   - destruct (to_val er') eqn:?.
     + destruct er'; simplify_eq/=.
       revert select (imp_link_prod_combine_ectx _ _ _ _ _ _ _ _) => HK.
       inversion HK; clear HK; simplify_eq/=.
       * tstep_i => *; destruct_all?; simplify_eq. tstep_s. split!.
-        apply Hloop. by split!.
+        apply: Hloop; [done|]. by split!.
       * tstep_i => *; destruct_all?; simplify_eq/=.
         tstep_i; split => *; simplify_eq.
-        apply Hloop. rewrite !expr_fill_app. split!; [done..|].
+        apply: Hloop; [done|]. rewrite !expr_fill_app. split!; [done..|].
         by apply static_expr_expr_fill.
     + tstep_both. apply: steps_impl_step_end => ?? /prim_step_inv[//|?[?[?[?[??]]]]] *.
       simplify_eq. revert select (Is_true (static_expr _ _)) => /static_expr_expr_fill/=[??]//.
       rewrite -expr_fill_app.
       invert_all head_step => //; destruct_all?; simplify_eq.
       * tstep_s => *. tend. split!; [done..|].
-        apply: Hloop. rewrite !expr_fill_app. split!; [done..| ].
+        apply: Hloop; [done|]. rewrite !expr_fill_app. split!; [done..| ].
         by apply static_expr_expr_fill.
       * tstep_s => *. tend. split!; [done..|].
-        apply: Hloop. rewrite !expr_fill_app. split!; [done..| ].
+        apply: Hloop; [done|]. rewrite !expr_fill_app. split!; [done..| ].
         by apply static_expr_expr_fill.
       * tstep_s => *. tend. split!; [done..|].
-        apply: Hloop. rewrite !expr_fill_app. split!; [done..| ].
+        apply: Hloop; [done|]. rewrite !expr_fill_app. split!; [done..| ].
         by apply static_expr_expr_fill.
       * tstep_s => *. split!;[done..|] => *. tend. split!; [done..|].
-        apply: Hloop. rewrite !expr_fill_app. split!; [done..| ].
+        apply: Hloop; [done|]. rewrite !expr_fill_app. split!; [done..| ].
         by apply static_expr_expr_fill.
       * tstep_s => *. tend. split!; [done..|].
-        apply: Hloop. rewrite !expr_fill_app. split!; [done..| ].
+        apply: Hloop; [done|]. rewrite !expr_fill_app. split!; [done..| ].
         by apply static_expr_expr_fill.
-      * tstep_s => b ?. subst. tend. split!. apply: Hloop. rewrite !expr_fill_app. split!; [done..| ].
+      * tstep_s => b ?. subst. tend. split!. apply: Hloop; [done|]. rewrite !expr_fill_app. split!; [done..| ].
         apply static_expr_expr_fill. split!. destruct b; naive_solver.
       * tstep_s => *. tend. split!; [done..|].
-        apply: Hloop. rewrite !expr_fill_app. split!; [done..| ].
+        apply: Hloop; [done|]. rewrite !expr_fill_app. split!; [done..| ].
         apply static_expr_expr_fill. split!. by apply static_expr_subst.
       * by tstep_s.
       * tstep_s. left. split!; [apply lookup_union_Some; naive_solver|] => ?. tend. split!; [done..|].
-        apply: Hloop. rewrite !expr_fill_app. split!; [done..|].
+        apply: Hloop; [done|]. rewrite !expr_fill_app. split!; [done..|].
         apply static_expr_expr_fill. split!. apply static_expr_subst_l; [|done].
         apply static_expr_mono. apply fd_static.
       * move => *. destruct_all?; simplify_eq/=. repeat case_bool_decide => //.
@@ -1232,10 +1383,10 @@ Proof.
            tstep_s. left. split!; [apply lookup_union_Some; naive_solver|] => ?.
            tend. split!.
            tstep_i. split => *; invert_all imp_prod_filter. case_bool_decide => //.
-           apply: Hloop. split!; [by econs|done..|].
+           apply: Hloop; [done|]. split!; [by econs|done..|].
            apply static_expr_subst_l; [|done]. apply static_expr_mono. apply fd_static.
         -- tstep_s. right. split!; [apply lookup_union_None;split!;by apply not_elem_of_dom|done|].
-           tend. split!. apply: Hloop. split!; [by econs|rewrite ?orb_true_r; done..].
+           tend. split!. apply: Hloop; [done|]. split!; [by econs|rewrite ?orb_true_r; done..].
   - tstep_i => *.
     repeat match goal with | x : imp_ev |- _ => destruct x end; simplify_eq/=; destruct_all?; simplify_eq/=.
     + tstep_s. left. repeat case_bool_decide => //.
@@ -1243,20 +1394,20 @@ Proof.
                [rewrite lookup_union_Some //; naive_solver |].
       * case_bool_decide. 2: { by tstep_s. }
         tstep_i. split => *; destruct_all?; simplify_eq/=. case_bool_decide => //.
-        apply Hloop. split!; [by econs|done..|]. apply static_expr_subst_l; [|done].
+        apply: Hloop; [done|]. split!; [by econs|done..|]. apply static_expr_subst_l; [|done].
         apply static_expr_mono. apply fd_static.
       * case_bool_decide. 2: { by tstep_s. }
         tstep_i. split => *; destruct_all?; simplify_eq/=. case_bool_decide => //.
-        apply Hloop. split!; [by econs|done..|]. apply static_expr_subst_l; [|done].
+        apply: Hloop; [done|]. split!; [by econs|done..|]. apply static_expr_subst_l; [|done].
         apply static_expr_mono. apply fd_static.
     + tstep_s. right.
       revert select (imp_link_prod_combine_ectx _ _ _ _ _ _ _ _) => HK.
       inversion HK; clear HK; simplify_eq; rewrite ?orb_true_r.
       * split!. tstep_i. split => *; destruct_all?; simplify_eq/=.
-        apply Hloop. rewrite !expr_fill_app. split!; [done|done..|].
+        apply: Hloop; [done|]. rewrite !expr_fill_app. split!; [done|done..|].
         by apply static_expr_expr_fill.
       * split!. tstep_i. split => *; destruct_all?; simplify_eq/=.
-        apply Hloop. rewrite !expr_fill_app. split!; [done|done..|].
+        apply: Hloop; [done|]. rewrite !expr_fill_app. split!; [done|done..|].
         by apply static_expr_expr_fill.
 Qed.
 
@@ -1273,784 +1424,4 @@ Proof.
   apply imp_prod_trefines; [apply _..| |].
   - apply: Href.
   - erewrite map_difference_eq_dom_L => //. apply _.
-Qed.
-
-
-(** * imp_heap_bij *)
-Record heap_bij := HeapBij {
-  hb_bij : gset (prov * prov);
-  hb_env : gset prov;
-  hb_prog : gset prov;
-  hb_disj_env : hb_env ## set_map snd hb_bij;
-  hb_disj_prog : hb_prog ## set_map snd hb_bij;
-  hb_disj_priv : hb_prog ## hb_env;
-  hb_iff p1 p2 p1' p2' : (p1, p2) ∈ hb_bij → (p1', p2') ∈ hb_bij → p1 = p1' ↔ p2 = p2'
-}.
-
-Global Program Instance imp_heap_bij_empty : Empty heap_bij :=
-  HeapBij ∅ ∅ ∅ _ _ _ _.
-Solve Obligations with set_solver.
-
-Definition hb_provs_right (bij : heap_bij) : gset prov :=
-  (set_map snd (hb_bij bij) ∪ hb_env bij ∪ hb_prog bij).
-
-Definition heap_bij_extend (p : player) (bij bij' : heap_bij) :=
-  hb_bij bij ⊆ hb_bij bij' ∧
-  (if p is Env then hb_env bij ⊆ hb_env bij' else hb_env bij = hb_env bij') ∧
-  (if p is Prog then hb_prog bij ⊆ hb_prog bij' else hb_prog bij = hb_prog bij').
-
-Global Instance heap_bij_extend_preorder p : PreOrder (heap_bij_extend p).
-Proof.
-  unfold heap_bij_extend. constructor.
-  - move => *. destruct p;set_solver.
-  - move => *. destruct p;set_solver.
-Qed.
-Global Typeclasses Opaque heap_bij_extend.
-
-Program Definition heap_bij_add_loc (p1 p2 : prov) (bij : heap_bij)
-        (H : p1 ∉ set_map (D:=gset _) fst (hb_bij bij)) (_ : p2 ∉ hb_provs_right bij) :=
-  HeapBij ({[ (p1, p2 )]} ∪ hb_bij bij) (hb_env bij) (hb_prog bij) _ _ _ _.
-Next Obligation.
-  move => ?????. rewrite set_map_union_L. apply disjoint_union_r. split; [|apply hb_disj_env].
-  rewrite set_map_singleton_L disjoint_singleton_r. set_solver.
-Qed.
-Next Obligation.
-  move => ?????. rewrite set_map_union_L. apply disjoint_union_r. split; [|apply hb_disj_prog].
-  rewrite set_map_singleton_L disjoint_singleton_r. set_solver.
-Qed.
-Next Obligation. move => *. apply hb_disj_priv. Qed.
-Next Obligation.
-  move => ??? Hl Hr??????. set_unfold.
-  destruct_all?; simplify_eq => //.
-  - split => ?;  [contradict Hl | contradict Hr; left; left]; eexists (_,_); naive_solver.
-  - split => ?;  [contradict Hl | contradict Hr; left; left]; eexists (_,_); naive_solver.
-  - by apply: hb_iff.
-Qed.
-
-(** ** val_in_bij *)
-Definition val_in_bij (bij : gset (prov * prov)) (v1 v2 : val) : Prop :=
-  match v1, v2 with
-  | ValNum n1, ValNum n2 => n1 = n2
-  | ValBool b1, ValBool b2 => b1 = b2
-  | ValLoc l1, ValLoc l2 => (l1.1, l2.1) ∈ bij /\ l1.2 = l2.2
-  | _, _ => False
-  end.
-
-Lemma val_in_bij_mono bij bij' v1 v2:
-  val_in_bij bij v1 v2 →
-  bij ⊆ bij' →
-  val_in_bij bij' v1 v2.
-Proof. destruct v1, v2 => //=. set_solver. Qed.
-
-(** ** expr_in_bij *)
-Fixpoint expr_in_bij (bij : gset (prov * prov)) (e1 e2 : expr) {struct e1} : Prop :=
-  match e1, e2 with
-  | Var v, Var v' => v = v'
-  | Val v, Val v' => val_in_bij bij v v'
-  | BinOp e1 o e2, BinOp e1' o' e2' => o = o' ∧ expr_in_bij bij e1 e1' ∧ expr_in_bij bij e2 e2'
-  | Load e, Load e' => expr_in_bij bij e e'
-  | Store e1 e2, Store e1' e2' => expr_in_bij bij e1 e1' ∧ expr_in_bij bij e2 e2'
-  | Alloc e, Alloc e' => expr_in_bij bij e e'
-  | Free e, Free e' => expr_in_bij bij e e'
-  | If e e1 e2, If e' e1' e2' => expr_in_bij bij e e' ∧ expr_in_bij bij e1 e1' ∧ expr_in_bij bij e2 e2'
-  | LetE v e1 e2, LetE v' e1' e2' => v = v' ∧ expr_in_bij bij e1 e1' ∧ expr_in_bij bij e2 e2'
-  | Call f args, Call f' args' => f = f' ∧ length args = length args' ∧
-                                   Forall id (zip_with (expr_in_bij bij) args args')
-  | UbE, UbE => True
-  | ReturnExt b e, ReturnExt b' e' => b = b' ∧ expr_in_bij bij e e'
-  | Waiting b, Waiting b' => b = b'
-  | _, _ => False
-  end.
-
-Lemma Forall2_bij_val_inv_l bij vl el :
-  Forall2 (expr_in_bij bij) (Val <$> vl) el →
-  ∃ vl', el = Val <$> vl' ∧ Forall2 (val_in_bij bij) vl vl'.
-Proof.
-  elim: vl el; csimpl. { move => ? /Forall2_nil_inv_l->. by eexists []. }
-  move => ?? IH ? /(Forall2_cons_inv_l _ _)[v' [?[?[/IH[?[??]]?]]]]; subst.
-  destruct v' => //. eexists (_::_). split; [done|]. by econs.
-Qed.
-
-Lemma Forall2_bij_val_inv_r bij vl el :
-  Forall2 (expr_in_bij bij) el (Val <$> vl) →
-  ∃ vl', el = Val <$> vl' ∧ Forall2 (val_in_bij bij) vl' vl.
-Proof.
-  elim: vl el; csimpl. { move => ? /Forall2_nil_inv_r->. by eexists []. }
-  move => ?? IH ? /(Forall2_cons_inv_r _ _ _ _) [v' [?[?[/IH[?[??]] ?]]]]; subst.
-  destruct v' => //. eexists (_::_). split; [done|]. by econs.
-Qed.
-
-Lemma expr_in_bij_mono bij bij' e1 e2:
-  expr_in_bij bij e1 e2 →
-  bij ⊆ bij' →
-  expr_in_bij bij' e1 e2.
-Proof.
-  elim: e1 e2 => //=*; repeat case_match => //; try naive_solver (eauto using val_in_bij_mono).
-  destruct_all?; simplify_eq. split!.
-  revert select (Forall id _). generalize dependent args.
-  revert select (Forall _ _). elim. { by case. }
-  move => ????? []//=??? *; decompose_Forall_hyps. econs; naive_solver.
-Qed.
-
-Lemma expr_in_bij_subst bij x v e v' e':
-  expr_in_bij bij e e' →
-  val_in_bij bij v v' →
-  expr_in_bij bij (subst x v e) (subst x v' e').
-Proof.
-  elim: e e' => //= *; repeat (case_match => //); simplify_eq/=; repeat case_bool_decide => //; try naive_solver.
-  destruct_all?. rewrite !fmap_length. split!.
-  revert select (Forall _ _). generalize dependent args.
-  revert select (Forall _ _). elim. { by case. }
-  move => ????? []//=??? /(Forall_cons_1 _ _)[??]. econs; naive_solver.
-Qed.
-
-Lemma expr_in_bij_subst_l bij xs vs e vs' e':
-  expr_in_bij bij e e' →
-  Forall2 (val_in_bij bij) vs vs' →
-  length xs = length vs →
-  expr_in_bij bij (subst_l xs vs e) (subst_l xs vs' e').
-Proof.
-  move => He Hall. elim: Hall xs e e' He. { by case. }
-  move => ?????? IH []//=??????. apply: IH; [|lia]. by apply expr_in_bij_subst.
-Qed.
-
-Lemma expr_in_bij_static bij e:
-  static_expr false e →
-  expr_in_bij bij e e.
-Proof.
-  elim: e => //=; try naive_solver. { by case. }
-  move => ?? IH Hb. split!.
-  elim: IH Hb => //=; econs; naive_solver.
-Qed.
-
-(** ** ectx_in_bij *)
-Definition ectx_item_in_bij (bij : gset (prov * prov)) (Ki Ki' : expr_ectx) : Prop :=
-  match Ki, Ki' with
-  | BinOpLCtx op e2, BinOpLCtx op' e2' => op = op' ∧ expr_in_bij bij e2 e2'
-  | BinOpRCtx v1 op, BinOpRCtx v1' op' => op = op' ∧ val_in_bij bij v1 v1'
-  | LoadCtx, LoadCtx => True
-  | StoreLCtx e2, StoreLCtx e2' => expr_in_bij bij e2 e2'
-  | StoreRCtx v1, StoreRCtx v1' => val_in_bij bij v1 v1'
-  | AllocCtx, AllocCtx => True
-  | FreeCtx, FreeCtx => True
-  | IfCtx e2 e3, IfCtx e2' e3' => expr_in_bij bij e2 e2' ∧ expr_in_bij bij e3 e3'
-  | LetECtx v e2, LetECtx v' e2' => v = v' ∧ expr_in_bij bij e2 e2'
-  | CallCtx f vl el, CallCtx f' vl' el' => f = f' ∧ Forall2 (val_in_bij bij) vl vl' ∧
-                                            Forall2 (expr_in_bij bij) el el'
-  | ReturnExtCtx b, ReturnExtCtx b' => b = b'
-  | _, _ => False
-  end.
-
-Definition ectx_in_bij (bij : gset (prov * prov)) (K1 K2 : list expr_ectx) : Prop :=
-  Forall2 (ectx_item_in_bij bij) K1 K2.
-
-Lemma ectx_item_in_bij_mono bij bij' K1 K2:
-  ectx_item_in_bij bij K1 K2 →
-  bij ⊆ bij' →
-  ectx_item_in_bij bij' K1 K2.
-Proof.
-  destruct K1, K2 => //=; try naive_solver (eauto using expr_in_bij_mono, val_in_bij_mono).
-  move => [?[??]] ?. split_and!; [done|..].
-  all: apply: Forall2_impl; [done|]; eauto using expr_in_bij_mono, val_in_bij_mono.
-Qed.
-
-Lemma ectx_in_bij_mono bij bij' K1 K2:
-  ectx_in_bij bij K1 K2 →
-  bij ⊆ bij' →
-  ectx_in_bij bij' K1 K2.
-Proof. move => ??. apply: Forall2_impl; [done|]. move => *; by apply: ectx_item_in_bij_mono.  Qed.
-
-Lemma ectx_in_bij_cons bij Ki K Ki' K':
-  ectx_in_bij bij (Ki :: K) (Ki' :: K') ↔ ectx_item_in_bij bij Ki Ki' ∧ ectx_in_bij bij K K'.
-Proof. apply Forall2_cons. Qed.
-
-Lemma ectx_in_bij_app bij Ki K Ki' K':
-  ectx_in_bij bij Ki Ki' →
-  ectx_in_bij bij K K' →
-  ectx_in_bij bij (Ki ++ K) (Ki' ++ K').
-Proof. apply Forall2_app. Qed.
-
-Lemma ectx_in_bij_cons_inv_l bij Ki K K':
-  ectx_in_bij bij (Ki::K) K' →
-  ∃ Ki' K'', ectx_item_in_bij bij Ki Ki' ∧ ectx_in_bij bij K K'' ∧ K' = Ki' :: K''.
-Proof. apply Forall2_cons_inv_l. Qed.
-
-Lemma expr_in_bij_fill_item_2 bij K1 K2 e1 e2 :
-  ectx_item_in_bij bij K1 K2 →
-  expr_in_bij bij e1 e2 →
-  expr_in_bij bij (expr_fill_item K1 e1) (expr_fill_item K2 e2).
-Proof.
-  move => ??.
-  destruct K1, K2 => //; simplify_eq/=; destruct_all? => //.
-  rewrite !app_length /=. split_and!; [done|solve_length|].
-  apply Forall_zip_with_2. apply Forall2_app; [by apply Forall2_fmap|by econs].
-Qed.
-
-Lemma expr_in_bij_fill_2 bij K1 K2 e1 e2 :
-  ectx_in_bij bij K1 K2 →
-  expr_in_bij bij e1 e2 →
-  expr_in_bij bij (expr_fill K1 e1) (expr_fill K2 e2).
-Proof.
-  elim: K1 K2 e1 e2. { move => ??? /Forall2_nil_inv_l->. done. }
-  move => Ki1 K1 IH ??? /(Forall2_cons_inv_l _ _)[Ki2 [K2 [?[??]]]] ?; subst => /=.
-  apply: IH; [done|]. by apply expr_in_bij_fill_item_2.
-Qed.
-
-Lemma expr_in_bij_fill_item_l bij Ki e1 e2 :
-  expr_in_bij bij (expr_fill_item Ki e1) e2 →
-  ∃ Ki' e', e2 = expr_fill_item Ki' e' ∧ ectx_item_in_bij bij Ki Ki' ∧ expr_in_bij bij e1 e'.
-Proof.
-  destruct Ki, e2 => //= *; destruct_all?; simplify_eq; try case_match => //; simplify_eq. 10: {
-    revert select (Forall _ _) => /Forall_zip_with_1 Hall.
-    move: (Hall ltac:(done)) => /Forall2_app_inv_l[?[?[Hv[/(Forall2_cons_inv_l _ _)[?[?[?[??]]]]?]]]]. simplify_eq.
-    move: Hv => /Forall2_bij_val_inv_l[?[??]]. simplify_eq.
-    by eexists (CallCtx _ _ _), _.
-  }
-  all: (unshelve eexists _); [econs; shelve| naive_solver].
-Qed.
-
-Lemma expr_in_bij_fill_l bij K e1 e2 :
-  expr_in_bij bij (expr_fill K e1) e2 →
-  ∃ K' e', e2 = expr_fill K' e' ∧ ectx_in_bij bij K K' ∧ expr_in_bij bij e1 e'.
-Proof.
-  elim: K e1 e2 => /=. { move => *. eexists [], _. split!. econs. }
-  move => Ki K IH e1 e2 /IH[K'[?[?[?/expr_in_bij_fill_item_l?]]]].
-  destruct_all?; simplify_eq. eexists (_ :: _), _ => /=. split_and!; [done| |done].
-  by econs.
-Qed.
-
-Lemma eval_binop_bij o v1 v2 v1' v2' v bij:
-  eval_binop o v1 v2 = Some v →
-  val_in_bij bij v1' v1 →
-  val_in_bij bij v2' v2 →
-  ∃ v', eval_binop o v1' v2' = Some v' ∧
-       val_in_bij bij v' v.
-Proof.
-  destruct o, v1, v2, v1', v2' => //= *; destruct_all?; simplify_eq. all: split!.
-  lia.
-Qed.
-
-(** *** heap_in_bij *)
-Definition heap_in_bij (bij : gset (prov * prov)) (h h' : heap_state) : Prop :=
-  ∀ p1 p2 o,
-  (p1, p2) ∈ bij →
-
-  (is_Some (h.(h_heap) !! (p1, o)) ↔ is_Some (h'.(h_heap) !! (p2, o)))
-  /\
-  ∀ v1 v2,
-  h.(h_heap)  !! (p1, o) = Some v1 →
-  h'.(h_heap) !! (p2, o) = Some v2 →
-  val_in_bij bij v1 v2.
-
-Lemma heap_in_bij_alive bij h1 h2 l1 l2:
-  heap_in_bij bij h1 h2 →
-  heap_alive h2 l2 →
-  (l1.1, l2.1) ∈ bij →
-  l1.2 = l2.2 →
-  heap_alive h1 l1.
-Proof.
-  move => ? Hbij ??. destruct l1 as [p1 ?], l2 as [p2 o]; simplify_eq/=.
-  unfold heap_in_bij, heap_alive in *. naive_solver.
-Qed.
-
-Lemma heap_in_bij_lookup bij h1 h2 l1 l2 v:
-  h_heap h2 !! l2 = Some v →
-  heap_in_bij bij h1 h2 →
-  (l1.1, l2.1) ∈ bij →
-  l1.2 = l2.2 →
-  ∃ v', h_heap h1 !! l1 = Some v' ∧ val_in_bij bij v' v.
-Proof.
-  move => ? Hbij ??. destruct l1 as [p1 ?], l2 as [p2 o]; simplify_eq/=.
-  have [[? H2]?]:= Hbij _ _ o ltac:(done).
-  have [??]:= H2 ltac:(done).
-  naive_solver.
-Qed.
-
-Lemma heap_in_bij_update bij h1 h2 l1 l2 v1 v2:
-  heap_in_bij (hb_bij bij) h1 h2 →
-  val_in_bij (hb_bij bij) v1 v2 →
-  (l1.1, l2.1) ∈ (hb_bij bij) →
-  l1.2 = l2.2 →
-  heap_in_bij (hb_bij bij) (heap_update h1 l1 v1) (heap_update h2 l2 v2).
-Proof.
-  move => Hbij ???. destruct l1 as [p1 ?], l2 as [p2 o]; simplify_eq/=.
-  move => p1' p2' o' /=?. have : p1 = p1' ↔ p2 = p2' by apply: hb_iff.
-  split.
-  - rewrite !lookup_alter_is_Some. by apply Hbij.
-  - move => ?? /lookup_alter_Some[[?[?[??]]]|[??]] /lookup_alter_Some[[?[?[??]]]|[??]]; simplify_eq.
-    all: try by eapply Hbij. all: naive_solver.
-Qed.
-
-Lemma heap_in_bij_alloc l1 l2 hi hs n bij H1 H2:
-  heap_in_bij (hb_bij bij) hi hs →
-  heap_is_fresh hi l1 →
-  heap_is_fresh hs l2 →
-  heap_in_bij (hb_bij (heap_bij_add_loc l1.1 l2.1 bij H1 H2)) (heap_alloc hi l1 n) (heap_alloc hs l2 n).
-Proof.
-  move => /= Hbij [Hi1 ?] [Hi2 ?] p1 p2 o /= /elem_of_union[?|?].
-  - set_unfold; simplify_eq. destruct l1 as [p1 ?], l2 as [p2 ?]; simplify_eq/=.
-    rewrite !lookup_union_l'.
-    { apply eq_None_ne_Some => ??. apply Hi1. by apply: (heap_wf _ (_, _)). }
-    { apply eq_None_ne_Some => ??. apply Hi2. by apply: (heap_wf _ (_, _)). }
-    split.
-    + rewrite !list_to_map_lookup_is_Some. f_equiv => ?. rewrite !elem_of_list_fmap. f_equiv => ?. naive_solver.
-    + move => ?? /(elem_of_list_to_map_2 _ _ _)/elem_of_list_fmap[?[??]].
-      move => /(elem_of_list_to_map_2 _ _ _)/elem_of_list_fmap[?[??]]. by simplify_eq/=.
-  - have ? : p1 ≠ l1.1 by contradict H1; set_unfold; eexists (_, _); naive_solver.
-    have ? : p2 ≠ l2.1 by contradict H2; set_unfold; left; left; eexists (_, _); naive_solver.
-    have [Hbij1 Hbij2]:= Hbij p1 p2 o ltac:(set_solver).
-    rewrite !lookup_union_r.
-    1, 2: apply not_elem_of_list_to_map_1;
-        move => /elem_of_list_fmap[[[??]?] [?/elem_of_list_fmap[?[??]]]]; simplify_eq/=.
-    split; [done|] => *. apply: val_in_bij_mono; [naive_solver|]. set_solver.
-Qed.
-
-
-Lemma heap_in_bij_free hi hs l1 l2 bij:
-  heap_in_bij (hb_bij bij) hi hs →
-  (l1.1, l2.1) ∈ hb_bij bij →
-  heap_in_bij (hb_bij bij) (heap_free hi l1) (heap_free hs l2).
-Proof.
-  move => Hbij Hin p1 p2 o /=?.
-  have [Hbij1 Hbij2]:= Hbij p1 p2 o ltac:(done).
-  have ?: p1 = l1.1 ↔ p2 = l2.1 by apply: hb_iff.
-  split.
-  - rewrite !map_filter_lookup /=. destruct (h_heap hi !! (p1, o)), (h_heap hs !! (p2, o)) => //=.
-    all: repeat case_option_guard => //; naive_solver.
-  - move => ??. rewrite !map_filter_lookup => /bind_Some[?[??]] /bind_Some[?[??]].
-    repeat case_option_guard => //; naive_solver.
-Qed.
-
-(** *** heap_preserved *)
-Definition heap_preserved (ps : gset prov) (h h' : heap_state) :=
-  ∀ p o, p ∈ ps → h.(h_heap) !! (p, o) = h'.(h_heap) !! (p, o).
-
-Global Instance heap_preserved_equivalence ps : Equivalence (heap_preserved ps).
-Proof.
-  unfold heap_preserved. constructor.
-  - done.
-  - move => ???. naive_solver.
-  - move => ??? Hp1 Hp2 ???. etrans; [by apply Hp1|]. by apply Hp2.
-Qed.
-
-Lemma heap_preserved_mono ps1 ps2 h h':
-  heap_preserved ps1 h h' →
-  ps2 ⊆ ps1 →
-  heap_preserved ps2 h h'.
-Proof. unfold heap_preserved => Hp ????. apply: Hp. set_solver. Qed.
-
-Lemma heap_preserved_bij_env p1 p2 l v he hp bij:
-  (p1, p2) ∈ hb_bij bij →
-  l.1 = p2 →
-  heap_preserved (hb_env bij) he hp →
-  heap_preserved (hb_env bij) he (heap_update hp l v).
-Proof.
-  move => ?? Hp p o /=?. destruct (decide (l = (p, o))); subst; simplify_map_eq.
-  - exfalso. have := hb_disj_env bij. apply; [done|]. apply elem_of_map. by eexists (_, _).
-  - by apply Hp.
-Qed.
-
-Lemma heap_preserved_bij_env_free p1 p2 l he hp bij:
-  (p1, p2) ∈ hb_bij bij →
-  l.1 = p2 →
-  heap_preserved (hb_env bij) he hp →
-  heap_preserved (hb_env bij) he (heap_free hp l).
-Proof.
-  move => ?? Hp p o /=?. rewrite map_filter_lookup. etrans; [by apply Hp|].
-  destruct (h_heap hp !! (p, o)) => //=. case_option_guard => //.
-  exfalso. have := hb_disj_env bij. apply; [done|]. apply elem_of_map. eexists (_, _). naive_solver.
-Qed.
-
-Lemma heap_preserved_bij_env_alloc l n he hp bij:
-  l.1 ∉ bij →
-  heap_preserved bij he hp →
-  heap_preserved bij he (heap_alloc hp l n).
-Proof.
-  move => Hni Hp p o /= ?. rewrite lookup_union_r; [| by apply Hp].
-  apply not_elem_of_list_to_map_1 => /elem_of_list_fmap[[[??]?] [?/elem_of_list_fmap[?[??]]]]; simplify_eq/=.
-  done.
-Qed.
-
-Record imp_heap_bij_state := ImpHeapBij {
-  ihb_bij : heap_bij;
-  (* last seen heap *)
-  ihb_heap : heap_state;
-}.
-Add Printing Constructor imp_heap_bij_state.
-
-Definition imp_heap_bij_pre (e : imp_event) (s : imp_heap_bij_state) : prepost (imp_event * imp_heap_bij_state) :=
-  let ho := heap_of_event e.2 in
-  pp_quant $ λ bij',
-  pp_quant $ λ vsi,
-  pp_quant $ λ hi,
-  pp_prop (heap_bij_extend Env s.(ihb_bij) bij') $
-  (* TODO: should we also have the following for hi? We don't need it so far... *)
-  pp_prop (set_map fst (hb_bij bij') ⊆ h_provs ho) $
-  pp_prop (Forall2 (val_in_bij (hb_bij bij')) (vals_of_event e.2) vsi) $
-  pp_prop (heap_in_bij (hb_bij bij') ho hi) $
-  pp_prop (heap_preserved (hb_prog bij') s.(ihb_heap) hi) $
-  pp_end ((e.1, event_set_vals_heap e.2 vsi hi), ImpHeapBij bij' hi).
-
-Definition imp_heap_bij_post (e : imp_event) (s : imp_heap_bij_state) : prepost (imp_event * imp_heap_bij_state) :=
-  let hi := heap_of_event e.2 in
-  pp_quant $ λ bij',
-  pp_quant $ λ vso,
-  pp_quant $ λ ho,
-  pp_prop (heap_bij_extend Prog s.(ihb_bij) bij') $
-  (* TODO: should we also have the following for hi? We don't need it so far... *)
-  pp_prop (set_map fst (hb_bij bij') ⊆ h_provs ho) $
-  pp_prop (Forall2 (val_in_bij (hb_bij bij')) vso (vals_of_event e.2)) $
-  pp_prop (heap_in_bij (hb_bij bij') ho hi) $
-  pp_prop (heap_preserved (hb_env bij') s.(ihb_heap) hi) $
-  pp_end ((e.1, event_set_vals_heap e.2 vso ho), ImpHeapBij bij' hi).
-
-Definition imp_heap_bij (m : module imp_event) : module imp_event :=
-  mod_prepost imp_heap_bij_pre imp_heap_bij_post m.
-
-Definition initial_imp_heap_bij_state (m : module imp_event) (σ : m.(m_state)) :=
-  (@SMFilter imp_event, σ, (@PPOutside imp_event imp_event, ImpHeapBij ∅ initial_heap_state)).
-
-Local Ltac split_solve :=
-  match goal with
-  | |- heap_in_bij ?p _ _ => is_evar p; eassumption
-  | |- event_set_vals_heap _ _ _ = event_set_vals_heap _ _ _ => reflexivity
-  | |- heap_bij_extend ?p ?a ?b =>
-      assert_fails (has_evar p); assert_fails (has_evar a); assert_fails (has_evar b); by etrans
-  | |- ?a ⊆ ?b =>
-      assert_fails (has_evar a); assert_fails (has_evar b); etrans; [eassumption|]
-  | |- ?a ⊆ ?b =>
-      assert_fails (has_evar a); assert_fails (has_evar b); etrans; [|eassumption]
-  | |- heap_preserved ?p ?a ?b =>
-      assert_fails (has_evar p); assert_fails (has_evar a); assert_fails (has_evar b); etrans; [eassumption|]
-  end.
-Local Ltac split_tac ::=
-  repeat (original_split_tac; try split_solve).
-
-Lemma imp_heap_bij_combine fns1 fns2 m1 m2 σ1 σ2 `{!VisNoAll m1} `{!VisNoAll m2}:
-  trefines (MS (imp_prod fns1 fns2 (imp_heap_bij m1) (imp_heap_bij m2))
-               (MLFNone, [], initial_imp_heap_bij_state m1 σ1,
-                 initial_imp_heap_bij_state m2 σ2))
-           (MS (imp_heap_bij (imp_prod fns1 fns2 m1 m2))
-               (initial_imp_heap_bij_state (imp_prod _ _ _ _)
-                  (MLFNone, [], σ1, σ2) )
-).
-Proof.
-  unshelve apply: mod_prepost_link. { exact
-      (λ ips '(ImpHeapBij bij1 hi1) '(ImpHeapBij bij2 hi2) '(ImpHeapBij bij hi) ics1 ics2,
-        ∃ bijm,
-          ics1 = ics2 ∧
-          hb_bij bij1 ⊆ bijm ∧
-          hb_bij bij2 ⊆ bijm ∧
-          hb_bij bij ⊆ bijm ∧
-       ((ips = SPNone ∧ bijm = hb_bij bij ∧
-          hb_env bij1 ⊆ hb_env bij ∪ hb_prog bij2 ∧
-          hb_env bij2 ⊆ hb_env bij ∪ hb_prog bij1 ∧
-          hb_prog bij = hb_prog bij1 ∪ hb_prog bij2 ∧
-          hb_prog bij1 ## hb_prog bij2 ∧
-          heap_preserved (hb_prog bij1) hi1 hi ∧
-          heap_preserved (hb_prog bij2) hi2 hi) ∨
-        ((ips = SPLeft ∧ bijm = hb_bij bij1 ∧
-          hb_env bij1 = hb_env bij ∪ hb_prog bij2 ∧
-          hb_env bij2 ⊆ hb_env bij ∪ hb_prog bij1 ∧
-          hb_prog bij ⊆ hb_prog bij1 ∪ hb_prog bij2 ∧
-          hb_prog bij2 ## hb_env bij ∧
-          heap_preserved (hb_env bij) hi hi1 ∧
-          heap_preserved (hb_prog bij2) hi2 hi1) ∨
-         (ips = SPRight ∧ bijm = hb_bij bij2 ∧
-          hb_env bij1 ⊆ hb_env bij ∪ hb_prog bij2 ∧
-          hb_env bij2 = hb_env bij ∪ hb_prog bij1 ∧
-          hb_prog bij ⊆ hb_prog bij1 ∪ hb_prog bij2 ∧
-          hb_prog bij1 ## hb_env bij ∧
-          heap_preserved (hb_env bij) hi hi2 ∧
-          heap_preserved (hb_prog bij1) hi1 hi2)))). }
-  { move => ?? [] /=*; naive_solver. }
-  { split!. all: set_solver. }
-  all: move => [bij1 hi1] [bij2 hi2] [bij hi] ics1 ics2.
-  - move => e ics' e' /= *. unfold heap_bij_extend in *; destruct_all?; simplify_eq/=.
-    unshelve split!. 1: econstructor. all: shelve_unifiable. all: split!. all: split!.
-    1: { set_unfold; naive_solver. }
-    1: { apply: heap_preserved_mono; [done|]. set_unfold; naive_solver. }
-    1: by destruct e.
-    1: { set_unfold; naive_solver. }
-    1: { set_unfold; naive_solver. }
-    1: { apply: disjoint_mono; [apply hb_disj_priv| |done]. set_unfold; naive_solver. }
-    1: { apply: heap_preserved_mono; [done|]. set_unfold; naive_solver. }
-  - move => e ics' e' /= *. unfold heap_bij_extend in *; destruct_all?; simplify_eq/=.
-    unshelve split!. 1: econstructor. all: shelve_unifiable. all: split!. all: split!.
-    1: { set_unfold; naive_solver. }
-    1: { apply: heap_preserved_mono; [done|]. set_unfold; naive_solver. }
-    1: by destruct e.
-    1: { set_unfold; naive_solver. }
-    1: { set_unfold; naive_solver. }
-    1: { apply: disjoint_mono; [apply hb_disj_priv| |done]. set_unfold; naive_solver. }
-    1: { apply: heap_preserved_mono; [done|]. set_unfold; naive_solver. }
-  - move => [? e] /= *. unfold heap_bij_extend in *; destruct_all?; simplify_eq/=.
-    unshelve split!. 1: econstructor. all: shelve_unifiable.
-    all: split!; rewrite ?heap_of_event_event_set_vals_heap; split!. all: split!.
-    1: { set_unfold; naive_solver. }
-    1: { rewrite vals_of_event_event_set_vals_heap //. by apply: Forall2_length. }
-    1: { apply: heap_preserved_mono; [done|]. set_unfold; naive_solver. }
-    1: { set_unfold; naive_solver. }
-    1: { set_unfold; naive_solver. }
-    1: { apply: disjoint_mono; [apply hb_disj_priv|done|]. set_unfold; naive_solver. }
-    1: { apply: heap_preserved_mono; [done|]. set_unfold; naive_solver. }
-    1: by destruct e.
-    1: by destruct e.
-  - move => [? e] /= *. unfold heap_bij_extend in *; destruct_all?; simplify_eq/=.
-    unshelve split!. 1: econstructor. all: shelve_unifiable.
-    all: split!; rewrite ?heap_of_event_event_set_vals_heap; split!. all: split!.
-    1: by destruct e.
-    1: { set_unfold; naive_solver. }
-    1: { apply: heap_preserved_mono; [done|]. set_unfold; naive_solver. }
-    1: { set_unfold; naive_solver. }
-    1: { set_unfold; naive_solver. }
-    1: { apply: disjoint_mono; [apply hb_disj_priv|done|]. set_unfold; naive_solver. }
-    1: { apply: heap_preserved_mono; [done|]. set_unfold; naive_solver. }
-  - move => [? e] /= *. unfold heap_bij_extend in *; destruct_all?; simplify_eq/=.
-    unshelve split!. 1: econstructor. all: shelve_unifiable.
-    all: split!; rewrite ?heap_of_event_event_set_vals_heap; split!. all: split!.
-    1: { set_unfold; naive_solver. }
-    1: { rewrite vals_of_event_event_set_vals_heap //. by apply: Forall2_length. }
-    1: { apply: heap_preserved_mono; [done|]. set_unfold; naive_solver. }
-    1: { set_unfold; naive_solver. }
-    1: { set_unfold; naive_solver. }
-    1: { apply: disjoint_mono; [apply hb_disj_priv|done|]. set_unfold; naive_solver. }
-    1: { apply: heap_preserved_mono; [done|]. set_unfold; naive_solver. }
-    1: by destruct e.
-    1: by destruct e.
-  - move => [? e] /= *. unfold heap_bij_extend in *; destruct_all?; simplify_eq/=.
-    unshelve split!. 1: econstructor. all: shelve_unifiable.
-    all: split!; rewrite ?heap_of_event_event_set_vals_heap; split!. all: split!.
-    1: by destruct e.
-    1: { set_unfold; naive_solver. }
-    1: { apply: heap_preserved_mono; [done|]. set_unfold; naive_solver. }
-    1: { set_unfold; naive_solver. }
-    1: { set_unfold; naive_solver. }
-    1: { symmetry. apply: disjoint_mono; [apply hb_disj_priv|done|]. set_unfold; naive_solver. }
-    1: { apply: heap_preserved_mono; [done|]. set_unfold; naive_solver. }
-    Unshelve.
-    (* We need to use abstract here as otherwise Qed does not terminate. *)
-    all: try abstract (by apply hb_iff).
-    all: abstract (
-      try (apply disjoint_union_l; split);
-      try (apply disjoint_union_r; split);
-      try (by apply hb_disj_env);
-      try (by apply hb_disj_prog);
-      try done;
-      try (apply: disjoint_mono; [apply hb_disj_prog| |done]; apply: subseteq_mono_eq_r; [|eassumption]);
-      try (apply: disjoint_mono; [apply hb_disj_priv| |done]; apply: subseteq_mono_eq_r; [|eassumption]);
-      try (apply: disjoint_mono; [apply hb_disj_env| |done]; apply: subseteq_mono_eq_r; [|eassumption]);
-      try (apply: disjoint_mono; [apply hb_disj_priv|done|]; apply: subseteq_mono_eq_r; [|eassumption]);
-      try (symmetry; apply: disjoint_mono; [apply hb_disj_priv|done|]; apply: subseteq_mono_eq_r; [|eassumption]);
-      set_unfold; naive_solver).
-Qed.
-
-Inductive imp_heap_bij_refl_ectx :
-  nat → (* paramater of previous waiting *) bool → @pp_state imp_event imp_event → list expr_ectx → Prop :=
-| IHBRE_Nil:
-  imp_heap_bij_refl_ectx 0 false PPOutside []
-| IHBRE_Return n b K:
-  imp_heap_bij_refl_ectx n b PPOutside K →
-  imp_heap_bij_refl_ectx (S n) true PPInside (ReturnExtCtx b :: K)
-| IHBRE_Ctx b n K K':
-  imp_heap_bij_refl_ectx n b PPInside K →
-  static_expr true (expr_fill K' (Var "")) →
-  imp_heap_bij_refl_ectx (S n) true PPOutside (K' ++ K)
-.
-
-Local Ltac split_solve ::=
-  match goal with
-  | |- expr_fill (?K' ++ ?K) _ = expr_fill ?K _ =>
-      assert_fails (has_evar K'); assert_fails (has_evar K); apply expr_fill_app
-  | |- expr_fill ?K _ = expr_fill ?K _ =>
-      assert_fails (has_evar K); reflexivity
-  | |- Is_true (static_expr _ (expr_fill _ _)) => apply static_expr_expr_fill
-  | |- expr_in_bij ?b (expr_fill _ _) (expr_fill _ _) =>
-      assert_fails (has_evar b); apply expr_in_bij_fill_2
-  | |- ectx_in_bij ?b (_ ++ _) (_ ++ _) => assert_fails (has_evar b); by apply ectx_in_bij_app
-  end.
-Local Ltac split_tac ::=
-  repeat (original_split_tac; try split_solve).
-
-(* Local Ltac split_tac ::= original_split_tac. *)
-
-Lemma imp_heap_bij_imp_refl fns:
-  trefines (MS imp_module (initial_imp_state fns))
-           (MS (imp_heap_bij imp_module)
-               (initial_imp_heap_bij_state imp_module (initial_imp_state fns))).
-Proof.
-  unshelve apply: inv_implies_trefines. { simpl. exact (λ '(Imp ei hi fnsi) '(ips, Imp es hs fnss, (pp, ImpHeapBij bij he)),
-    ∃ bij' n Ki ei' b,
-    fnsi = fns ∧ fnss = fns ∧
-    imp_heap_bij_refl_ectx n b pp Ki ∧
-    hb_env bij = hb_env bij' ∧
-    hb_prog bij = ∅ ∧ hb_prog bij' = ∅ ∧
-    heap_preserved (hb_env bij') he hs ∧
-    ei = expr_fill Ki ei' ∧
-    expr_in_bij (hb_bij bij') ei es ∧
-    heap_in_bij (hb_bij bij') hi hs ∧
-    set_map fst (hb_bij bij') ⊆ h_provs hi ∧
-    match pp with
-    | PPOutside =>
-        ei' = Waiting b ∧ ips = SMFilter ∧ hb_bij bij = hb_bij bij'
-    | PPInside =>
-        hb_bij bij ⊆ hb_bij bij' ∧
-        static_expr true ei' ∧ ips = SMProg
-    | _ => False
-    end
- ). }
-  { eexists ∅. split!. econs. done. }
-  move => /= [ei hi fnsi] [[ips [es hs fnss]] [pp [bij he]]] ??? Hprim. destruct_all?; simplify_eq.
-  revert select (expr_in_bij _ (expr_fill _ _) _) => /expr_in_bij_fill_l[?[?[?[??]]]].
-  case_match; destruct_all?; simplify_eq.
-  - move: Hprim => /prim_step_inv_head[|//|??]. { solve_sub_redexes_are_values. } destruct_all?; simplify_eq.
-    invert_all @head_step; destruct_all?; simplify_eq.
-    + case_match => //; simplify_eq. tstep_s. split!; [done|]. tstep_s. move => *. tstep_s. split!.
-      case_bool_decide. 2: { by tstep_s. }
-      tend. case_bool_decide => //. 2: solve_length.
-      unfold heap_bij_extend in *.
-      split!. 1: by econs. 1: done. all: split!.
-      1, 2: set_solver.
-      1: { apply: ectx_in_bij_mono; [done|set_solver]. }
-      1: { apply expr_in_bij_subst_l; [|done|solve_length]. apply expr_in_bij_static. apply fd_static. }
-      apply static_expr_subst_l => //. apply static_expr_mono. apply fd_static.
-    + case_match => //; simplify_eq. tstep_s. split!; [done|]. tstep_s. move => *. tstep_s. split!. tend.
-      revert select (imp_heap_bij_refl_ectx _ _ _ _) => HK.
-      inversion HK; clear HK; simplify_eq/=.
-      unfold heap_bij_extend in *.
-      split!. 1: done. 1: done. all: split!. 1, 2: set_solver.
-      1: { apply: ectx_in_bij_mono; [done|set_solver]. }
-      by decompose_Forall_hyps.
-  - destruct (to_val ei') eqn:?.
-    + destruct ei'; simplify_eq/=.
-      revert select (imp_heap_bij_refl_ectx _ _ _ _) => HK.
-      inversion HK; clear HK; simplify_eq/=.
-      move: Hprim => /prim_step_inv_head[|//|??]. { solve_sub_redexes_are_values. } destruct_all?; simplify_eq.
-      case_match => //; simplify_eq/=.
-      revert select (ectx_in_bij _ (_ :: _) _) => /ectx_in_bij_cons_inv_l[Ki'[?[?[??]]]]; simplify_eq.
-      destruct Ki' => //; simplify_eq/=.
-      invert_all @head_step; destruct_all?; simplify_eq.
-      tstep_s. tstep_s.
-      eexists bij'. split!. 1: split; split!; set_solver. 1: done. 1: econs; [done|econs]. 1: done. 1: done. tend.
-      split!. 1: done. 1: reflexivity. all: split!.
-    + move: Hprim => /prim_step_inv[//|??]. destruct_all?; simplify_eq.
-      revert select (expr_in_bij _ (expr_fill _ _) _) => /expr_in_bij_fill_l[?[?[?[??]]]].
-      revert select (Is_true (static_expr _ _)) => /static_expr_expr_fill/=[??]//.
-      invert_all @head_step; destruct_all?; simplify_eq.
-      all: repeat (case_match; destruct_all? => //); simplify_eq.
-      * tstep_s => ? /eval_binop_bij Hbin. have [?[??]]:= Hbin _ _ _ ltac:(done) ltac:(done).
-        tend. split!. 1: done. 1: done. all: split!.
-      * tstep_s => *; simplify_eq/=. destruct v1 => //; simplify_eq/=; destruct_all?; simplify_eq/=. tend.
-        have [//|?[??]]:= heap_in_bij_lookup _ _ _ _ _ _ ltac:(done) ltac:(done) ltac:(done).
-        split!. 1: done. 1: done. 1: done. all: split!.
-      * tstep_s => *; simplify_eq/=. destruct v1 => //; simplify_eq/=; destruct_all?; simplify_eq/=. tend.
-        split!. 1: by apply: heap_in_bij_alive. 1: done. 1: done. all: split!.
-        1: by apply: heap_preserved_bij_env.
-        1: by apply heap_in_bij_update.
-      * tstep_s => *; simplify_eq/=.
-        set (l' := (heap_fresh (hb_provs_right bij') hs)).
-        eexists l'. split; [apply heap_fresh_is_fresh|] => *; simplify_eq/=. tend.
-        destruct v => //; simplify_eq/=; destruct_all?; simplify_eq/=.
-        split!. 1: done.
-        unshelve instantiate (1:=(heap_bij_add_loc l.1 l'.1 bij' _ _)).
-        { abstract (apply: not_elem_of_weaken; [|done]; unfold heap_is_fresh in *; naive_solver). }
-        { apply: heap_fresh_not_in. }
-        all: split!.
-        1: { apply heap_preserved_bij_env_alloc; [|done] => ?.
-             apply: (heap_fresh_not_in (hb_provs_right bij') hs). set_solver. }
-        1: { apply: ectx_in_bij_mono; [by apply ectx_in_bij_app|set_solver]. }
-        1: set_solver.
-        1: unfold heap_is_fresh in *; naive_solver.
-        1: { apply: (heap_in_bij_alloc l l').
-             { abstract (apply: not_elem_of_weaken; [|done]; unfold heap_is_fresh in *; naive_solver). }
-             { apply: heap_fresh_not_in. }
-          done. done. apply heap_fresh_is_fresh. }
-        1: set_solver.
-        1: set_solver.
-      * tstep_s => *; simplify_eq/=. tend.
-        destruct v => //; simplify_eq/=; destruct_all?; simplify_eq/=.
-        split!. 1: by apply: heap_in_bij_alive. 1: done. 1: done. all: split!.
-        1: by apply: heap_preserved_bij_env_free.
-        1: by apply heap_in_bij_free.
-      * tstep_s => *; simplify_eq/=. destruct v => //; simplify_eq/=. tend.
-        split!. 1: done. 1: done. all: split!. all: by case_match.
-      * tstep_s. tend. split!. 1: done. 1: done. all: split!.
-        1: by apply expr_in_bij_subst.
-        1: by apply static_expr_subst.
-      * tstep_s. done.
-      * revert select (Forall id _) => /Forall_zip_with_1 Hall.
-        move: (Hall ltac:(done)) => /Forall2_bij_val_inv_l[?[??]]; simplify_eq.
-        tstep_s. left. split! => *. tend.
-        split!. 1: solve_length. 1: done. 1: done. all: split!.
-        1: { apply expr_in_bij_subst_l; [|done|solve_length]. apply expr_in_bij_static. apply fd_static. }
-        apply static_expr_subst_l; [|solve_length]. apply static_expr_mono. apply fd_static.
-      * revert select (Forall id _) => /Forall_zip_with_1 Hall.
-        move: (Hall ltac:(done)) => /Forall2_bij_val_inv_l[?[??]]; simplify_eq.
-        simplify_eq. tstep_s. right. split! => *. tstep_s.
-        eexists bij'. split!. 1: split; split!; set_solver. 1,2,3,4: done. tend.
-        split!. 1: by apply: IHBRE_Ctx. 1: reflexivity. all: split!.
-Qed.
-
-Lemma imp_heap_bij_imp_closed m σ:
-  trefines (MS (imp_closed (imp_heap_bij m)) (SMFilter, initial_imp_heap_bij_state m σ, ICStart))
-           (MS (imp_closed m) (SMFilter, σ, ICStart)).
-Proof.
-  apply tsim_implies_trefines => /= n.
-  unshelve apply: tsim_remember. { simpl. exact (λ _
-          '(σm1, (σf, σ1, (pp, ImpHeapBij bij hi)), σc1)
-          '(σm2, σ2, σc2),
-           σ1 = σ2 ∧ σc1 = σc2 ∧
-             ((σc1 = ICStart ∧ σf = SMFilter ∧ pp = PPOutside ∧ σm1 = σm2 ∧ σm2 = SMFilter ∧ bij = ∅) ∨
-              ( ((∃ e, σf = SMProgRecv e ∧ σm2 = SMProgRecv e) ∨ (σf = SMProg ∧ σm2 = SMProg)
-                 ) ∧ σm1 = SMProg ∧ σc1 = ICRunning ∧ pp = PPInside))
-                             ). }
-  { split!. } { done. }
-  move => {}n _ /= Hloop [[σm1 [[σf σ1] [pp [bij hi]]]] σc1] [[σm2 σ2] σc2] ?. destruct_all?; simplify_eq/=.
-  - tstep_i. apply steps_impl_step_end => ???. invert_all' @m_step; simplify_eq/=. split!.
-    tstep_s. eexists (Some (inr _)). split!. apply: steps_spec_step_end; [econs|] => ??. simplify_eq/=.
-    tstep_i. apply steps_impl_step_end => ???. invert_all @m_step. split!.
-    tstep_s. eexists (Some (inl _)). split!. apply: steps_spec_step_end; [econs|] => ??. simplify_eq/=.
-    tstep_i => ??; simplify_eq/=.
-    tstep_i. eexists ∅, (ValNum <$> vs), initial_heap_state. split!.
-    1: { apply Forall2_fmap. apply Forall_Forall2_diag. by apply Forall_true. }
-    apply: Hloop. split!.
-  - tstep_both. apply steps_impl_step_end => κ ??. case_match => *; simplify_eq.
-    + tstep_s.  eexists (Some _). split; [done|]. apply: steps_spec_step_end; [done|] => ??. tend. split!; [done|].
-      apply: Hloop. split!.
-    + tstep_s. eexists None. apply: steps_spec_step_end; [done|] => ??. tend. split!; [done|].
-      apply: Hloop. split!.
-  - tstep_both. apply steps_impl_step_end => κ ??. tstep_s. eexists _. apply: steps_spec_step_end; [done|] => ??.
-    case_match; tend; (split!; [done|]). 2: { apply: Hloop. split!. }
-    tstep_i => ? vs *. tstep_both => *.
-    apply steps_impl_step_end => ???. invert_all @m_step => ?; simplify_eq.
-    + destruct i as [? [? vs' |]]; simplify_eq/=.
-      tstep_s. eexists (Some _). split!.
-      apply: steps_spec_step_end; [econs|]=> /=??. destruct_all?; simplify_eq/=. tend.
-      split!.
-      tstep_both. apply steps_impl_step_end => ???. invert_all @m_step.
-      tstep_s. eexists (None). apply: steps_spec_step_end; [econs|]=> /=??. destruct_all?; simplify_eq/=. tend.
-      have ?: vs0 = ValNum <$> vs'0. {
-        revert select (m_step _ _ _ _) => _.
-        revert select (Forall2 _ _ _). elim: vs'0 vs0; csimpl => *; decompose_Forall_hyps => //.
-        match goal with |- ?x :: _ = _ => destruct x; simplify_eq/= => // end. naive_solver.
-      } subst.
-      split!; [done|].
-      tstep_i. apply steps_impl_step_end => ???. invert_all @m_step. split!.
-      tstep_s. eexists (Some (inr _)). split!. apply: steps_spec_step_end; [econs|] => /=? ->.
-      tstep_i. apply steps_impl_step_end => ???. invert_all @m_step. split!.
-      tstep_s. eexists (Some (inl _)). split!. apply: steps_spec_step_end; [econs|] => /=? ->.
-      tstep_i => ? <-.
-      tstep_i. eexists _, [ValNum _]. split!. 1: done. 1: done. 1: econs; [done|econs]. 1: done. 1: done.
-      apply: Hloop. split!.
-    + destruct i as [? []]; simplify_eq/=.
-      tstep_s. eexists (Some _). split!.
-      apply: steps_spec_step_end; [econs|]=> /=??. destruct_all?; simplify_eq/=.
-      tstep_s. eexists None. apply: steps_spec_step_end; [econs|]=> /=??. destruct_all?; simplify_eq/=.
-      destruct vs as [|v ?]; decompose_Forall_hyps. destruct v => //; simplify_eq/=.
-      tend. split!.
-      tstep_i. apply: steps_impl_step_end => ???. invert_all @m_step. split!.
-      tstep_i. apply: steps_impl_step_end => ???. invert_all @m_step. split!.
-      tstep_s. eexists (Some (inr _)). split!.
-      apply: steps_spec_step_end; [econs|]=> /=? ->.
-      tstep_i. apply: steps_impl_step_end => ???. invert_all @m_step.
 Qed.
