theories/imp_heap_bij.v
@@ -1,0 +1,806 @@
+Require Export refframe.module.
+Require Import refframe.trefines.
+Require Import refframe.filter.
+Require Import refframe.product.
+Require Import refframe.seq_product.
+Require Import refframe.link.
+Require Import refframe.prepost.
+Require Import refframe.proof_techniques.
+Require Import refframe.imp.
+
+(** * imp_heap_bij *)
+Record heap_bij := HeapBij {
+  hb_bij : gset (prov * prov);
+  hb_env : gset prov;
+  hb_prog : gset prov;
+  hb_disj_env : hb_env ## set_map snd hb_bij;
+  hb_disj_prog : hb_prog ## set_map snd hb_bij;
+  hb_disj_priv : hb_prog ## hb_env;
+  hb_iff p1 p2 p1' p2' : (p1, p2) ∈ hb_bij → (p1', p2') ∈ hb_bij → p1 = p1' ↔ p2 = p2'
+}.
+
+Global Program Instance imp_heap_bij_empty : Empty heap_bij :=
+  HeapBij ∅ ∅ ∅ _ _ _ _.
+Solve Obligations with set_solver.
+
+Definition hb_provs_right (bij : heap_bij) : gset prov :=
+  (set_map snd (hb_bij bij) ∪ hb_env bij ∪ hb_prog bij).
+
+Definition heap_bij_extend (p : player) (bij bij' : heap_bij) :=
+  hb_bij bij ⊆ hb_bij bij' ∧
+  (if p is Env then hb_env bij ⊆ hb_env bij' else hb_env bij = hb_env bij') ∧
+  (if p is Prog then hb_prog bij ⊆ hb_prog bij' else hb_prog bij = hb_prog bij').
+
+Global Instance heap_bij_extend_preorder p : PreOrder (heap_bij_extend p).
+Proof.
+  unfold heap_bij_extend. constructor.
+  - move => *. destruct p;set_solver.
+  - move => *. destruct p;set_solver.
+Qed.
+Global Typeclasses Opaque heap_bij_extend.
+
+Program Definition heap_bij_add_loc (p1 p2 : prov) (bij : heap_bij)
+        (H : p1 ∉ set_map (D:=gset _) fst (hb_bij bij)) (_ : p2 ∉ hb_provs_right bij) :=
+  HeapBij ({[ (p1, p2 )]} ∪ hb_bij bij) (hb_env bij) (hb_prog bij) _ _ _ _.
+Next Obligation.
+  move => ?????. rewrite set_map_union_L. apply disjoint_union_r. split; [|apply hb_disj_env].
+  rewrite set_map_singleton_L disjoint_singleton_r. set_solver.
+Qed.
+Next Obligation.
+  move => ?????. rewrite set_map_union_L. apply disjoint_union_r. split; [|apply hb_disj_prog].
+  rewrite set_map_singleton_L disjoint_singleton_r. set_solver.
+Qed.
+Next Obligation. move => *. apply hb_disj_priv. Qed.
+Next Obligation.
+  move => ??? Hl Hr??????. set_unfold.
+  destruct_all?; simplify_eq => //.
+  - split => ?;  [contradict Hl | contradict Hr; left; left]; eexists (_,_); naive_solver.
+  - split => ?;  [contradict Hl | contradict Hr; left; left]; eexists (_,_); naive_solver.
+  - by apply: hb_iff.
+Qed.
+
+(** ** val_in_bij *)
+Definition val_in_bij (bij : gset (prov * prov)) (v1 v2 : val) : Prop :=
+  match v1, v2 with
+  | ValNum n1, ValNum n2 => n1 = n2
+  | ValBool b1, ValBool b2 => b1 = b2
+  | ValLoc l1, ValLoc l2 => (l1.1, l2.1) ∈ bij /\ l1.2 = l2.2
+  | _, _ => False
+  end.
+
+Lemma val_in_bij_mono bij bij' v1 v2:
+  val_in_bij bij v1 v2 →
+  bij ⊆ bij' →
+  val_in_bij bij' v1 v2.
+Proof. destruct v1, v2 => //=. set_solver. Qed.
+
+(** ** expr_in_bij *)
+Fixpoint expr_in_bij (bij : gset (prov * prov)) (e1 e2 : expr) {struct e1} : Prop :=
+  match e1, e2 with
+  | Var v, Var v' => v = v'
+  | Val v, Val v' => val_in_bij bij v v'
+  | BinOp e1 o e2, BinOp e1' o' e2' => o = o' ∧ expr_in_bij bij e1 e1' ∧ expr_in_bij bij e2 e2'
+  | Load e, Load e' => expr_in_bij bij e e'
+  | Store e1 e2, Store e1' e2' => expr_in_bij bij e1 e1' ∧ expr_in_bij bij e2 e2'
+  | Alloc e, Alloc e' => expr_in_bij bij e e'
+  | Free e, Free e' => expr_in_bij bij e e'
+  | If e e1 e2, If e' e1' e2' => expr_in_bij bij e e' ∧ expr_in_bij bij e1 e1' ∧ expr_in_bij bij e2 e2'
+  | LetE v e1 e2, LetE v' e1' e2' => v = v' ∧ expr_in_bij bij e1 e1' ∧ expr_in_bij bij e2 e2'
+  | Call f args, Call f' args' => f = f' ∧ length args = length args' ∧
+                                   Forall id (zip_with (expr_in_bij bij) args args')
+  | UbE, UbE => True
+  | ReturnExt b e, ReturnExt b' e' => b = b' ∧ expr_in_bij bij e e'
+  | Waiting b, Waiting b' => b = b'
+  | _, _ => False
+  end.
+
+Lemma Forall2_bij_val_inv_l bij vl el :
+  Forall2 (expr_in_bij bij) (Val <$> vl) el →
+  ∃ vl', el = Val <$> vl' ∧ Forall2 (val_in_bij bij) vl vl'.
+Proof.
+  elim: vl el; csimpl. { move => ? /Forall2_nil_inv_l->. by eexists []. }
+  move => ?? IH ? /(Forall2_cons_inv_l _ _)[v' [?[?[/IH[?[??]]?]]]]; subst.
+  destruct v' => //. eexists (_::_). split; [done|]. by econs.
+Qed.
+
+Lemma Forall2_bij_val_inv_r bij vl el :
+  Forall2 (expr_in_bij bij) el (Val <$> vl) →
+  ∃ vl', el = Val <$> vl' ∧ Forall2 (val_in_bij bij) vl' vl.
+Proof.
+  elim: vl el; csimpl. { move => ? /Forall2_nil_inv_r->. by eexists []. }
+  move => ?? IH ? /(Forall2_cons_inv_r _ _ _ _) [v' [?[?[/IH[?[??]] ?]]]]; subst.
+  destruct v' => //. eexists (_::_). split; [done|]. by econs.
+Qed.
+
+Lemma expr_in_bij_mono bij bij' e1 e2:
+  expr_in_bij bij e1 e2 →
+  bij ⊆ bij' →
+  expr_in_bij bij' e1 e2.
+Proof.
+  elim: e1 e2 => //=*; repeat case_match => //; try naive_solver (eauto using val_in_bij_mono).
+  destruct_all?; simplify_eq. split!.
+  revert select (Forall id _). generalize dependent args.
+  revert select (Forall _ _). elim. { by case. }
+  move => ????? []//=??? *; decompose_Forall_hyps. econs; naive_solver.
+Qed.
+
+Lemma expr_in_bij_subst bij x v e v' e':
+  expr_in_bij bij e e' →
+  val_in_bij bij v v' →
+  expr_in_bij bij (subst x v e) (subst x v' e').
+Proof.
+  elim: e e' => //= *; repeat (case_match => //); simplify_eq/=; repeat case_bool_decide => //; try naive_solver.
+  destruct_all?. rewrite !fmap_length. split!.
+  revert select (Forall _ _). generalize dependent args.
+  revert select (Forall _ _). elim. { by case. }
+  move => ????? []//=??? /(Forall_cons_1 _ _)[??]. econs; naive_solver.
+Qed.
+
+Lemma expr_in_bij_subst_l bij xs vs e vs' e':
+  expr_in_bij bij e e' →
+  Forall2 (val_in_bij bij) vs vs' →
+  length xs = length vs →
+  expr_in_bij bij (subst_l xs vs e) (subst_l xs vs' e').
+Proof.
+  move => He Hall. elim: Hall xs e e' He. { by case. }
+  move => ?????? IH []//=??????. apply: IH; [|lia]. by apply expr_in_bij_subst.
+Qed.
+
+Lemma expr_in_bij_static bij e:
+  static_expr false e →
+  expr_in_bij bij e e.
+Proof.
+  elim: e => //=; try naive_solver. { by case. }
+  move => ?? IH Hb. split!.
+  elim: IH Hb => //=; econs; naive_solver.
+Qed.
+
+(** ** ectx_in_bij *)
+Definition ectx_item_in_bij (bij : gset (prov * prov)) (Ki Ki' : expr_ectx) : Prop :=
+  match Ki, Ki' with
+  | BinOpLCtx op e2, BinOpLCtx op' e2' => op = op' ∧ expr_in_bij bij e2 e2'
+  | BinOpRCtx v1 op, BinOpRCtx v1' op' => op = op' ∧ val_in_bij bij v1 v1'
+  | LoadCtx, LoadCtx => True
+  | StoreLCtx e2, StoreLCtx e2' => expr_in_bij bij e2 e2'
+  | StoreRCtx v1, StoreRCtx v1' => val_in_bij bij v1 v1'
+  | AllocCtx, AllocCtx => True
+  | FreeCtx, FreeCtx => True
+  | IfCtx e2 e3, IfCtx e2' e3' => expr_in_bij bij e2 e2' ∧ expr_in_bij bij e3 e3'
+  | LetECtx v e2, LetECtx v' e2' => v = v' ∧ expr_in_bij bij e2 e2'
+  | CallCtx f vl el, CallCtx f' vl' el' => f = f' ∧ Forall2 (val_in_bij bij) vl vl' ∧
+                                            Forall2 (expr_in_bij bij) el el'
+  | ReturnExtCtx b, ReturnExtCtx b' => b = b'
+  | _, _ => False
+  end.
+
+Definition ectx_in_bij (bij : gset (prov * prov)) (K1 K2 : list expr_ectx) : Prop :=
+  Forall2 (ectx_item_in_bij bij) K1 K2.
+
+Lemma ectx_item_in_bij_mono bij bij' K1 K2:
+  ectx_item_in_bij bij K1 K2 →
+  bij ⊆ bij' →
+  ectx_item_in_bij bij' K1 K2.
+Proof.
+  destruct K1, K2 => //=; try naive_solver (eauto using expr_in_bij_mono, val_in_bij_mono).
+  move => [?[??]] ?. split_and!; [done|..].
+  all: apply: Forall2_impl; [done|]; eauto using expr_in_bij_mono, val_in_bij_mono.
+Qed.
+
+Lemma ectx_in_bij_mono bij bij' K1 K2:
+  ectx_in_bij bij K1 K2 →
+  bij ⊆ bij' →
+  ectx_in_bij bij' K1 K2.
+Proof. move => ??. apply: Forall2_impl; [done|]. move => *; by apply: ectx_item_in_bij_mono.  Qed.
+
+Lemma ectx_in_bij_cons bij Ki K Ki' K':
+  ectx_in_bij bij (Ki :: K) (Ki' :: K') ↔ ectx_item_in_bij bij Ki Ki' ∧ ectx_in_bij bij K K'.
+Proof. apply Forall2_cons. Qed.
+
+Lemma ectx_in_bij_app bij Ki K Ki' K':
+  ectx_in_bij bij Ki Ki' →
+  ectx_in_bij bij K K' →
+  ectx_in_bij bij (Ki ++ K) (Ki' ++ K').
+Proof. apply Forall2_app. Qed.
+
+Lemma ectx_in_bij_cons_inv_l bij Ki K K':
+  ectx_in_bij bij (Ki::K) K' →
+  ∃ Ki' K'', ectx_item_in_bij bij Ki Ki' ∧ ectx_in_bij bij K K'' ∧ K' = Ki' :: K''.
+Proof. apply Forall2_cons_inv_l. Qed.
+
+Lemma expr_in_bij_fill_item_2 bij K1 K2 e1 e2 :
+  ectx_item_in_bij bij K1 K2 →
+  expr_in_bij bij e1 e2 →
+  expr_in_bij bij (expr_fill_item K1 e1) (expr_fill_item K2 e2).
+Proof.
+  move => ??.
+  destruct K1, K2 => //; simplify_eq/=; destruct_all? => //.
+  rewrite !app_length /=. split_and!; [done|solve_length|].
+  apply Forall_zip_with_2. apply Forall2_app; [by apply Forall2_fmap|by econs].
+Qed.
+
+Lemma expr_in_bij_fill_2 bij K1 K2 e1 e2 :
+  ectx_in_bij bij K1 K2 →
+  expr_in_bij bij e1 e2 →
+  expr_in_bij bij (expr_fill K1 e1) (expr_fill K2 e2).
+Proof.
+  elim: K1 K2 e1 e2. { move => ??? /Forall2_nil_inv_l->. done. }
+  move => Ki1 K1 IH ??? /(Forall2_cons_inv_l _ _)[Ki2 [K2 [?[??]]]] ?; subst => /=.
+  apply: IH; [done|]. by apply expr_in_bij_fill_item_2.
+Qed.
+
+Lemma expr_in_bij_fill_item_l bij Ki e1 e2 :
+  expr_in_bij bij (expr_fill_item Ki e1) e2 →
+  ∃ Ki' e', e2 = expr_fill_item Ki' e' ∧ ectx_item_in_bij bij Ki Ki' ∧ expr_in_bij bij e1 e'.
+Proof.
+  destruct Ki, e2 => //= *; destruct_all?; simplify_eq; try case_match => //; simplify_eq. 10: {
+    revert select (Forall _ _) => /Forall_zip_with_1 Hall.
+    move: (Hall ltac:(done)) => /Forall2_app_inv_l[?[?[Hv[/(Forall2_cons_inv_l _ _)[?[?[?[??]]]]?]]]]. simplify_eq.
+    move: Hv => /Forall2_bij_val_inv_l[?[??]]. simplify_eq.
+    by eexists (CallCtx _ _ _), _.
+  }
+  all: (unshelve eexists _); [econs; shelve| naive_solver].
+Qed.
+
+Lemma expr_in_bij_fill_l bij K e1 e2 :
+  expr_in_bij bij (expr_fill K e1) e2 →
+  ∃ K' e', e2 = expr_fill K' e' ∧ ectx_in_bij bij K K' ∧ expr_in_bij bij e1 e'.
+Proof.
+  elim: K e1 e2 => /=. { move => *. eexists [], _. split!. econs. }
+  move => Ki K IH e1 e2 /IH[K'[?[?[?/expr_in_bij_fill_item_l?]]]].
+  destruct_all?; simplify_eq. eexists (_ :: _), _ => /=. split_and!; [done| |done].
+  by econs.
+Qed.
+
+Lemma eval_binop_bij o v1 v2 v1' v2' v bij:
+  eval_binop o v1 v2 = Some v →
+  val_in_bij bij v1' v1 →
+  val_in_bij bij v2' v2 →
+  ∃ v', eval_binop o v1' v2' = Some v' ∧
+       val_in_bij bij v' v.
+Proof.
+  destruct o, v1, v2, v1', v2' => //= *; destruct_all?; simplify_eq. all: split!.
+  lia.
+Qed.
+
+(** *** heap_in_bij *)
+Definition heap_in_bij (bij : gset (prov * prov)) (h h' : heap_state) : Prop :=
+  ∀ p1 p2 o,
+  (p1, p2) ∈ bij →
+
+  (is_Some (h.(h_heap) !! (p1, o)) ↔ is_Some (h'.(h_heap) !! (p2, o)))
+  /\
+  ∀ v1 v2,
+  h.(h_heap)  !! (p1, o) = Some v1 →
+  h'.(h_heap) !! (p2, o) = Some v2 →
+  val_in_bij bij v1 v2.
+
+Lemma heap_in_bij_alive bij h1 h2 l1 l2:
+  heap_in_bij bij h1 h2 →
+  heap_alive h2 l2 →
+  (l1.1, l2.1) ∈ bij →
+  l1.2 = l2.2 →
+  heap_alive h1 l1.
+Proof.
+  move => ? Hbij ??. destruct l1 as [p1 ?], l2 as [p2 o]; simplify_eq/=.
+  unfold heap_in_bij, heap_alive in *. naive_solver.
+Qed.
+
+Lemma heap_in_bij_lookup bij h1 h2 l1 l2 v:
+  h_heap h2 !! l2 = Some v →
+  heap_in_bij bij h1 h2 →
+  (l1.1, l2.1) ∈ bij →
+  l1.2 = l2.2 →
+  ∃ v', h_heap h1 !! l1 = Some v' ∧ val_in_bij bij v' v.
+Proof.
+  move => ? Hbij ??. destruct l1 as [p1 ?], l2 as [p2 o]; simplify_eq/=.
+  have [[? H2]?]:= Hbij _ _ o ltac:(done).
+  have [??]:= H2 ltac:(done).
+  naive_solver.
+Qed.
+
+Lemma heap_in_bij_update bij h1 h2 l1 l2 v1 v2:
+  heap_in_bij (hb_bij bij) h1 h2 →
+  val_in_bij (hb_bij bij) v1 v2 →
+  (l1.1, l2.1) ∈ (hb_bij bij) →
+  l1.2 = l2.2 →
+  heap_in_bij (hb_bij bij) (heap_update h1 l1 v1) (heap_update h2 l2 v2).
+Proof.
+  move => Hbij ???. destruct l1 as [p1 ?], l2 as [p2 o]; simplify_eq/=.
+  move => p1' p2' o' /=?. have : p1 = p1' ↔ p2 = p2' by apply: hb_iff.
+  split.
+  - rewrite !lookup_alter_is_Some. by apply Hbij.
+  - move => ?? /lookup_alter_Some[[?[?[??]]]|[??]] /lookup_alter_Some[[?[?[??]]]|[??]]; simplify_eq.
+    all: try by eapply Hbij. all: naive_solver.
+Qed.
+
+Lemma heap_in_bij_alloc l1 l2 hi hs n bij H1 H2:
+  heap_in_bij (hb_bij bij) hi hs →
+  heap_is_fresh hi l1 →
+  heap_is_fresh hs l2 →
+  heap_in_bij (hb_bij (heap_bij_add_loc l1.1 l2.1 bij H1 H2)) (heap_alloc hi l1 n) (heap_alloc hs l2 n).
+Proof.
+  move => /= Hbij [Hi1 ?] [Hi2 ?] p1 p2 o /= /elem_of_union[?|?].
+  - set_unfold; simplify_eq. destruct l1 as [p1 ?], l2 as [p2 ?]; simplify_eq/=.
+    rewrite !lookup_union_l'.
+    { apply eq_None_ne_Some => ??. apply Hi1. by apply: (heap_wf _ (_, _)). }
+    { apply eq_None_ne_Some => ??. apply Hi2. by apply: (heap_wf _ (_, _)). }
+    split.
+    + rewrite !list_to_map_lookup_is_Some. f_equiv => ?. rewrite !elem_of_list_fmap. f_equiv => ?. naive_solver.
+    + move => ?? /(elem_of_list_to_map_2 _ _ _)/elem_of_list_fmap[?[??]].
+      move => /(elem_of_list_to_map_2 _ _ _)/elem_of_list_fmap[?[??]]. by simplify_eq/=.
+  - have ? : p1 ≠ l1.1 by contradict H1; set_unfold; eexists (_, _); naive_solver.
+    have ? : p2 ≠ l2.1 by contradict H2; set_unfold; left; left; eexists (_, _); naive_solver.
+    have [Hbij1 Hbij2]:= Hbij p1 p2 o ltac:(set_solver).
+    rewrite !lookup_union_r.
+    1, 2: apply not_elem_of_list_to_map_1;
+        move => /elem_of_list_fmap[[[??]?] [?/elem_of_list_fmap[?[??]]]]; simplify_eq/=.
+    split; [done|] => *. apply: val_in_bij_mono; [naive_solver|]. set_solver.
+Qed.
+
+
+Lemma heap_in_bij_free hi hs l1 l2 bij:
+  heap_in_bij (hb_bij bij) hi hs →
+  (l1.1, l2.1) ∈ hb_bij bij →
+  heap_in_bij (hb_bij bij) (heap_free hi l1) (heap_free hs l2).
+Proof.
+  move => Hbij Hin p1 p2 o /=?.
+  have [Hbij1 Hbij2]:= Hbij p1 p2 o ltac:(done).
+  have ?: p1 = l1.1 ↔ p2 = l2.1 by apply: hb_iff.
+  split.
+  - rewrite !map_filter_lookup /=. destruct (h_heap hi !! (p1, o)), (h_heap hs !! (p2, o)) => //=.
+    all: repeat case_option_guard => //; naive_solver.
+  - move => ??. rewrite !map_filter_lookup => /bind_Some[?[??]] /bind_Some[?[??]].
+    repeat case_option_guard => //; naive_solver.
+Qed.
+
+(** *** heap_preserved *)
+Definition heap_preserved (ps : gset prov) (h h' : heap_state) :=
+  ∀ p o, p ∈ ps → h.(h_heap) !! (p, o) = h'.(h_heap) !! (p, o).
+
+Global Instance heap_preserved_equivalence ps : Equivalence (heap_preserved ps).
+Proof.
+  unfold heap_preserved. constructor.
+  - done.
+  - move => ???. naive_solver.
+  - move => ??? Hp1 Hp2 ???. etrans; [by apply Hp1|]. by apply Hp2.
+Qed.
+
+Lemma heap_preserved_mono ps1 ps2 h h':
+  heap_preserved ps1 h h' →
+  ps2 ⊆ ps1 →
+  heap_preserved ps2 h h'.
+Proof. unfold heap_preserved => Hp ????. apply: Hp. set_solver. Qed.
+
+Lemma heap_preserved_bij_env p1 p2 l v he hp bij:
+  (p1, p2) ∈ hb_bij bij →
+  l.1 = p2 →
+  heap_preserved (hb_env bij) he hp →
+  heap_preserved (hb_env bij) he (heap_update hp l v).
+Proof.
+  move => ?? Hp p o /=?. destruct (decide (l = (p, o))); subst; simplify_map_eq.
+  - exfalso. have := hb_disj_env bij. apply; [done|]. apply elem_of_map. by eexists (_, _).
+  - by apply Hp.
+Qed.
+
+Lemma heap_preserved_bij_env_free p1 p2 l he hp bij:
+  (p1, p2) ∈ hb_bij bij →
+  l.1 = p2 →
+  heap_preserved (hb_env bij) he hp →
+  heap_preserved (hb_env bij) he (heap_free hp l).
+Proof.
+  move => ?? Hp p o /=?. rewrite map_filter_lookup. etrans; [by apply Hp|].
+  destruct (h_heap hp !! (p, o)) => //=. case_option_guard => //.
+  exfalso. have := hb_disj_env bij. apply; [done|]. apply elem_of_map. eexists (_, _). naive_solver.
+Qed.
+
+Lemma heap_preserved_bij_env_alloc l n he hp bij:
+  l.1 ∉ bij →
+  heap_preserved bij he hp →
+  heap_preserved bij he (heap_alloc hp l n).
+Proof.
+  move => Hni Hp p o /= ?. rewrite lookup_union_r; [| by apply Hp].
+  apply not_elem_of_list_to_map_1 => /elem_of_list_fmap[[[??]?] [?/elem_of_list_fmap[?[??]]]]; simplify_eq/=.
+  done.
+Qed.
+
+Record imp_heap_bij_state := ImpHeapBij {
+  ihb_bij : heap_bij;
+  (* last seen heap *)
+  ihb_heap : heap_state;
+}.
+Add Printing Constructor imp_heap_bij_state.
+
+Definition imp_heap_bij_pre (e : imp_event) (s : imp_heap_bij_state) : prepost (imp_event * imp_heap_bij_state) :=
+  let ho := heap_of_event e.2 in
+  pp_quant $ λ bij',
+  pp_quant $ λ vsi,
+  pp_quant $ λ hi,
+  pp_prop (heap_bij_extend Env s.(ihb_bij) bij') $
+  (* TODO: should we also have the following for hi? We don't need it so far... *)
+  pp_prop (set_map fst (hb_bij bij') ⊆ h_provs ho) $
+  pp_prop (Forall2 (val_in_bij (hb_bij bij')) (vals_of_event e.2) vsi) $
+  pp_prop (heap_in_bij (hb_bij bij') ho hi) $
+  pp_prop (heap_preserved (hb_prog bij') s.(ihb_heap) hi) $
+  pp_end ((e.1, event_set_vals_heap e.2 vsi hi), ImpHeapBij bij' hi).
+
+Definition imp_heap_bij_post (e : imp_event) (s : imp_heap_bij_state) : prepost (imp_event * imp_heap_bij_state) :=
+  let hi := heap_of_event e.2 in
+  pp_quant $ λ bij',
+  pp_quant $ λ vso,
+  pp_quant $ λ ho,
+  pp_prop (heap_bij_extend Prog s.(ihb_bij) bij') $
+  (* TODO: should we also have the following for hi? We don't need it so far... *)
+  pp_prop (set_map fst (hb_bij bij') ⊆ h_provs ho) $
+  pp_prop (Forall2 (val_in_bij (hb_bij bij')) vso (vals_of_event e.2)) $
+  pp_prop (heap_in_bij (hb_bij bij') ho hi) $
+  pp_prop (heap_preserved (hb_env bij') s.(ihb_heap) hi) $
+  pp_end ((e.1, event_set_vals_heap e.2 vso ho), ImpHeapBij bij' hi).
+
+Definition imp_heap_bij (m : module imp_event) : module imp_event :=
+  mod_prepost imp_heap_bij_pre imp_heap_bij_post m.
+
+Definition initial_imp_heap_bij_state (m : module imp_event) (σ : m.(m_state)) :=
+  (@SMFilter imp_event, σ, (@PPOutside imp_event imp_event, ImpHeapBij ∅ initial_heap_state)).
+
+Local Ltac split_solve :=
+  match goal with
+  | |- heap_in_bij ?p _ _ => is_evar p; eassumption
+  | |- event_set_vals_heap _ _ _ = event_set_vals_heap _ _ _ => reflexivity
+  | |- heap_bij_extend ?p ?a ?b =>
+      assert_fails (has_evar p); assert_fails (has_evar a); assert_fails (has_evar b); by etrans
+  | |- ?a ⊆ ?b =>
+      assert_fails (has_evar a); assert_fails (has_evar b); etrans; [eassumption|]
+  | |- ?a ⊆ ?b =>
+      assert_fails (has_evar a); assert_fails (has_evar b); etrans; [|eassumption]
+  | |- heap_preserved ?p ?a ?b =>
+      assert_fails (has_evar p); assert_fails (has_evar a); assert_fails (has_evar b); etrans; [eassumption|]
+  end.
+Local Ltac split_tac ::=
+  repeat (original_split_tac; try split_solve).
+
+Lemma imp_heap_bij_combine fns1 fns2 m1 m2 σ1 σ2 `{!VisNoAll m1} `{!VisNoAll m2}:
+  trefines (MS (imp_prod fns1 fns2 (imp_heap_bij m1) (imp_heap_bij m2))
+               (MLFNone, [], initial_imp_heap_bij_state m1 σ1,
+                 initial_imp_heap_bij_state m2 σ2))
+           (MS (imp_heap_bij (imp_prod fns1 fns2 m1 m2))
+               (initial_imp_heap_bij_state (imp_prod _ _ _ _)
+                  (MLFNone, [], σ1, σ2) )
+).
+Proof.
+  unshelve apply: mod_prepost_link. { exact
+      (λ ips '(ImpHeapBij bij1 hi1) '(ImpHeapBij bij2 hi2) '(ImpHeapBij bij hi) ics1 ics2,
+        ∃ bijm,
+          ics1 = ics2 ∧
+          hb_bij bij1 ⊆ bijm ∧
+          hb_bij bij2 ⊆ bijm ∧
+          hb_bij bij ⊆ bijm ∧
+       ((ips = SPNone ∧ bijm = hb_bij bij ∧
+          hb_env bij1 ⊆ hb_env bij ∪ hb_prog bij2 ∧
+          hb_env bij2 ⊆ hb_env bij ∪ hb_prog bij1 ∧
+          hb_prog bij = hb_prog bij1 ∪ hb_prog bij2 ∧
+          hb_prog bij1 ## hb_prog bij2 ∧
+          heap_preserved (hb_prog bij1) hi1 hi ∧
+          heap_preserved (hb_prog bij2) hi2 hi) ∨
+        ((ips = SPLeft ∧ bijm = hb_bij bij1 ∧
+          hb_env bij1 = hb_env bij ∪ hb_prog bij2 ∧
+          hb_env bij2 ⊆ hb_env bij ∪ hb_prog bij1 ∧
+          hb_prog bij ⊆ hb_prog bij1 ∪ hb_prog bij2 ∧
+          hb_prog bij2 ## hb_env bij ∧
+          heap_preserved (hb_env bij) hi hi1 ∧
+          heap_preserved (hb_prog bij2) hi2 hi1) ∨
+         (ips = SPRight ∧ bijm = hb_bij bij2 ∧
+          hb_env bij1 ⊆ hb_env bij ∪ hb_prog bij2 ∧
+          hb_env bij2 = hb_env bij ∪ hb_prog bij1 ∧
+          hb_prog bij ⊆ hb_prog bij1 ∪ hb_prog bij2 ∧
+          hb_prog bij1 ## hb_env bij ∧
+          heap_preserved (hb_env bij) hi hi2 ∧
+          heap_preserved (hb_prog bij1) hi1 hi2)))). }
+  { move => ?? [] /=*; naive_solver. }
+  { split!. all: set_solver. }
+  all: move => [bij1 hi1] [bij2 hi2] [bij hi] ics1 ics2.
+  - move => e ics' e' /= *. unfold heap_bij_extend in *; destruct_all?; simplify_eq/=.
+    unshelve split!. 1: econstructor. all: shelve_unifiable. all: split!. all: split!.
+    1: { set_unfold; naive_solver. }
+    1: { apply: heap_preserved_mono; [done|]. set_unfold; naive_solver. }
+    1: by destruct e.
+    1: { set_unfold; naive_solver. }
+    1: { set_unfold; naive_solver. }
+    1: { apply: disjoint_mono; [apply hb_disj_priv| |done]. set_unfold; naive_solver. }
+    1: { apply: heap_preserved_mono; [done|]. set_unfold; naive_solver. }
+  - move => e ics' e' /= *. unfold heap_bij_extend in *; destruct_all?; simplify_eq/=.
+    unshelve split!. 1: econstructor. all: shelve_unifiable. all: split!. all: split!.
+    1: { set_unfold; naive_solver. }
+    1: { apply: heap_preserved_mono; [done|]. set_unfold; naive_solver. }
+    1: by destruct e.
+    1: { set_unfold; naive_solver. }
+    1: { set_unfold; naive_solver. }
+    1: { apply: disjoint_mono; [apply hb_disj_priv| |done]. set_unfold; naive_solver. }
+    1: { apply: heap_preserved_mono; [done|]. set_unfold; naive_solver. }
+  - move => [? e] /= *. unfold heap_bij_extend in *; destruct_all?; simplify_eq/=.
+    unshelve split!. 1: econstructor. all: shelve_unifiable.
+    all: split!; rewrite ?heap_of_event_event_set_vals_heap; split!. all: split!.
+    1: { set_unfold; naive_solver. }
+    1: { rewrite vals_of_event_event_set_vals_heap //. by apply: Forall2_length. }
+    1: { apply: heap_preserved_mono; [done|]. set_unfold; naive_solver. }
+    1: { set_unfold; naive_solver. }
+    1: { set_unfold; naive_solver. }
+    1: { apply: disjoint_mono; [apply hb_disj_priv|done|]. set_unfold; naive_solver. }
+    1: { apply: heap_preserved_mono; [done|]. set_unfold; naive_solver. }
+    1: by destruct e.
+    1: by destruct e.
+  - move => [? e] /= *. unfold heap_bij_extend in *; destruct_all?; simplify_eq/=.
+    unshelve split!. 1: econstructor. all: shelve_unifiable.
+    all: split!; rewrite ?heap_of_event_event_set_vals_heap; split!. all: split!.
+    1: by destruct e.
+    1: { set_unfold; naive_solver. }
+    1: { apply: heap_preserved_mono; [done|]. set_unfold; naive_solver. }
+    1: { set_unfold; naive_solver. }
+    1: { set_unfold; naive_solver. }
+    1: { apply: disjoint_mono; [apply hb_disj_priv|done|]. set_unfold; naive_solver. }
+    1: { apply: heap_preserved_mono; [done|]. set_unfold; naive_solver. }
+  - move => [? e] /= *. unfold heap_bij_extend in *; destruct_all?; simplify_eq/=.
+    unshelve split!. 1: econstructor. all: shelve_unifiable.
+    all: split!; rewrite ?heap_of_event_event_set_vals_heap; split!. all: split!.
+    1: { set_unfold; naive_solver. }
+    1: { rewrite vals_of_event_event_set_vals_heap //. by apply: Forall2_length. }
+    1: { apply: heap_preserved_mono; [done|]. set_unfold; naive_solver. }
+    1: { set_unfold; naive_solver. }
+    1: { set_unfold; naive_solver. }
+    1: { apply: disjoint_mono; [apply hb_disj_priv|done|]. set_unfold; naive_solver. }
+    1: { apply: heap_preserved_mono; [done|]. set_unfold; naive_solver. }
+    1: by destruct e.
+    1: by destruct e.
+  - move => [? e] /= *. unfold heap_bij_extend in *; destruct_all?; simplify_eq/=.
+    unshelve split!. 1: econstructor. all: shelve_unifiable.
+    all: split!; rewrite ?heap_of_event_event_set_vals_heap; split!. all: split!.
+    1: by destruct e.
+    1: { set_unfold; naive_solver. }
+    1: { apply: heap_preserved_mono; [done|]. set_unfold; naive_solver. }
+    1: { set_unfold; naive_solver. }
+    1: { set_unfold; naive_solver. }
+    1: { symmetry. apply: disjoint_mono; [apply hb_disj_priv|done|]. set_unfold; naive_solver. }
+    1: { apply: heap_preserved_mono; [done|]. set_unfold; naive_solver. }
+    Unshelve.
+    (* We need to use abstract here as otherwise Qed does not terminate. *)
+    all: try abstract (by apply hb_iff).
+    all: abstract (
+      try (apply disjoint_union_l; split);
+      try (apply disjoint_union_r; split);
+      try (by apply hb_disj_env);
+      try (by apply hb_disj_prog);
+      try done;
+      try (apply: disjoint_mono; [apply hb_disj_prog| |done]; apply: subseteq_mono_eq_r; [|eassumption]);
+      try (apply: disjoint_mono; [apply hb_disj_priv| |done]; apply: subseteq_mono_eq_r; [|eassumption]);
+      try (apply: disjoint_mono; [apply hb_disj_env| |done]; apply: subseteq_mono_eq_r; [|eassumption]);
+      try (apply: disjoint_mono; [apply hb_disj_priv|done|]; apply: subseteq_mono_eq_r; [|eassumption]);
+      try (symmetry; apply: disjoint_mono; [apply hb_disj_priv|done|]; apply: subseteq_mono_eq_r; [|eassumption]);
+      set_unfold; naive_solver).
+Qed.
+
+
+Local Ltac split_solve ::=
+  match goal with
+  | |- expr_fill (?K' ++ ?K) _ = expr_fill ?K _ =>
+      assert_fails (has_evar K'); assert_fails (has_evar K); apply expr_fill_app
+  | |- expr_fill ?K _ = expr_fill ?K _ =>
+      assert_fails (has_evar K); reflexivity
+  | |- Is_true (static_expr _ (expr_fill _ _)) => apply static_expr_expr_fill
+  | |- expr_in_bij ?b (expr_fill _ _) (expr_fill _ _) =>
+      assert_fails (has_evar b); apply expr_in_bij_fill_2
+  | |- ectx_in_bij ?b (_ ++ _) (_ ++ _) => assert_fails (has_evar b); by apply ectx_in_bij_app
+  end.
+Local Ltac split_tac ::=
+  repeat (original_split_tac; try split_solve).
+
+Local Ltac bij_solver := unfold heap_bij_extend in *; set_unfold; naive_solver.
+
+Lemma imp_heap_bij_imp_refl fns:
+  trefines (MS imp_module (initial_imp_state fns))
+           (MS (imp_heap_bij imp_module)
+               (initial_imp_heap_bij_state imp_module (initial_imp_state fns))).
+Proof.
+  pose (R := λ (b : bool) '(ImpHeapBij bij1 h1) '(ImpHeapBij bij2 h2),
+          (hb_prog bij1 = ∅ → hb_prog bij2 = ∅) ∧ hb_bij bij1 ⊆ hb_bij bij2).
+  apply: (imp_prepost_proof R); unfold R in *.
+  { constructor. { move => [??]. naive_solver. }
+    { move => [??] [??] [??] [??] [??]. split. naive_solver. by etrans. } }
+  { move => [??] [??]. naive_solver. }
+  move => n K1 K2 f fn1 vs1 h1 [bij0 ?] ?? /= bij1 *.
+  split!. move => ?. split; [solve_length|].
+  move => Hcall Hret.
+  unshelve apply: tsim_remember. { simpl. exact (λ _ '(Imp ei hi fnsi) '(ips, Imp es hs fnss, (pp, ImpHeapBij bij he)),
+    (* bij' : current bijection, bij : bijection when last communicated with the environment,
+     bij1: bijection at the start of the function (necessary to reestablish R) *)
+    ∃ bij' ei' es',
+    fnsi = fns ∧ fnss = fns ∧
+    hb_env bij = hb_env bij' ∧
+    hb_prog bij = ∅ ∧ hb_prog bij' = ∅ ∧
+    hb_bij bij ⊆ hb_bij bij' ∧
+    hb_bij bij1 ⊆ hb_bij bij ∧
+    heap_preserved (hb_env bij') he hs ∧
+    ei = expr_fill K1 ei' ∧
+    es = expr_fill K2 es' ∧
+    expr_in_bij (hb_bij bij') ei' es' ∧
+    heap_in_bij (hb_bij bij') hi hs ∧
+    set_map fst (hb_bij bij') ⊆ h_provs hi ∧
+    pp = PPInside ∧
+    static_expr true ei' ∧
+    ips = SMProg
+ ). }
+  { eexists _. split!. done. all: split!.
+    { unfold heap_bij_extend in *. clear Hcall Hret. bij_solver. }
+    { unfold heap_bij_extend in *. clear Hcall Hret. bij_solver. }
+    { apply expr_in_bij_subst_l; [|done|solve_length]. apply expr_in_bij_static. apply fd_static. }
+    { apply static_expr_subst_l; [|solve_length]. apply static_expr_mono. apply fd_static. }  }
+  { naive_solver. }
+  move => /= n' ? Hloop [ei hi fnsi] [[ips [es hs fnss]] [pp [bij he]]] ?. destruct_all?; simplify_eq.
+  destruct (to_val ei') eqn:?.
+  - destruct ei' => //; simplify_eq/=. destruct es' => //; simplify_eq/=.
+    apply Hret; [done|]. clear Hloop Hret Hcall. split!.
+    { unfold heap_bij_extend. split!; [done..|]. bij_solver. }
+    all: split!. by econs. done.
+    { etrans; [|done]. etrans; [|done]. bij_solver. }
+  - (* TODO: remove this use of EM *)
+    have [?|?]:= EM (∃ K f vs, fns !! f = None ∧ ei' = expr_fill K (Call f (Val <$> vs))).
+    + destruct_all?; simplify_eq/=.
+      revert select (expr_in_bij _ (expr_fill _ _) _) => /expr_in_bij_fill_l[?[?[?[??]]]].
+      destruct_all?; simplify_eq/=.
+      revert select (Is_true (static_expr _ _)) => /static_expr_expr_fill/=[??]//.
+      case_match => //; destruct_all?; simplify_eq/=.
+      revert select (Forall id _) => /Forall_zip_with_1 Hall.
+      move: (Hall ltac:(done)) => /Forall2_bij_val_inv_l[?[??]]; simplify_eq.
+      apply: Hcall; [done..| | |].
+      1,2: by apply Forall2_fmap_l, Forall_Forall2_diag, Forall_true.
+      clear Hret. split!.
+      { unfold heap_bij_extend. split!; [done..|]. bij_solver. }
+      all: split!.
+      { etrans; [|done]. etrans; [|done]. bij_solver. }
+      move => ?? [??] *. decompose_Forall_hyps. split!.
+      apply Hloop; [done|]. split!. 1: done. all: split!.
+      1: bij_solver.
+      1: bij_solver.
+      { etrans; [done|]. etrans; [done|]. bij_solver. }
+      { apply: ectx_in_bij_mono; [done|]. bij_solver. }
+    + tstep_both.
+      apply steps_impl_step_end => ?? /= Hprim.
+      move: Hprim => /prim_step_inv[//|??].
+      destruct_all?; simplify_eq.
+      revert select (expr_in_bij _ (expr_fill _ _) _) => /expr_in_bij_fill_l[?[?[?[??]]]].
+      destruct_all?; simplify_eq.
+      revert select (Is_true (static_expr _ _)) => /static_expr_expr_fill/=[??]//.
+      invert_all' @head_step; destruct_all?; simplify_eq/=.
+      all: repeat (case_match; destruct_all? => //); simplify_eq.
+      * tstep_s => ? /eval_binop_bij Hbin. have [?[??]]:= Hbin _ _ _ ltac:(done) ltac:(done).
+        tend. split!. apply: Hloop; [done|]. split!. 1: done. 1: done. all: split!.
+      * tstep_s => *; simplify_eq/=. destruct v1 => //; simplify_eq/=; destruct_all?; simplify_eq/=. tend.
+        have [//|?[??]]:= heap_in_bij_lookup _ _ _ _ _ _ ltac:(done) ltac:(done) ltac:(done).
+        split!. 1: done.
+        apply: Hloop; [done|]. split!. 1: done. 1: done. all: split!.
+      * tstep_s => *; simplify_eq/=. destruct v1 => //; simplify_eq/=; destruct_all?; simplify_eq/=. tend.
+        split!. 1: by apply: heap_in_bij_alive.
+        apply: Hloop; [done|]. split!. 1: done. 1: done. all: split!.
+        1: by apply: heap_preserved_bij_env.
+        1: by apply heap_in_bij_update.
+      * tstep_s => *; simplify_eq/=.
+        set (l' := (heap_fresh (hb_provs_right bij') hs)).
+        eexists l'. split; [apply heap_fresh_is_fresh|] => *; simplify_eq/=. tend.
+        destruct v => //; simplify_eq/=; destruct_all?; simplify_eq/=.
+        split!.
+        apply Hloop; [done|].
+        unshelve eexists (heap_bij_add_loc l.1 l'.1 bij' _ _).
+        { abstract (apply: not_elem_of_weaken; [|done]; unfold heap_is_fresh in *; naive_solver). }
+        { apply: heap_fresh_not_in. }
+        split!.
+        1: bij_solver.
+        1: { apply heap_preserved_bij_env_alloc; [|done] => ?.
+             apply: (heap_fresh_not_in (hb_provs_right bij') hs). bij_solver. }
+        1: { apply: ectx_in_bij_mono; [done|bij_solver]. }
+        1: bij_solver.
+        1: unfold heap_is_fresh in *; naive_solver.
+        1: { apply: (heap_in_bij_alloc l l').
+             { abstract (apply: not_elem_of_weaken; [|done]; unfold heap_is_fresh in *; naive_solver). }
+             { apply: heap_fresh_not_in. }
+          done. done. apply heap_fresh_is_fresh. }
+        1: bij_solver.
+      * tstep_s => *; simplify_eq/=. tend.
+        destruct v => //; simplify_eq/=; destruct_all?; simplify_eq/=.
+        split!. 1: by apply: heap_in_bij_alive. apply: Hloop; [done|]. split!. 1: done. 1: done. all: split!.
+        1: by apply: heap_preserved_bij_env_free.
+        1: by apply heap_in_bij_free.
+      * tstep_s => *; simplify_eq/=. destruct v => //; simplify_eq/=. tend.
+        split!. apply: Hloop; [done|]. split!. 1: done. 1: done. all: split!. all: by case_match.
+      * tstep_s. tend. split!. apply: Hloop; [done|]. split!. 1: done. all: split!.
+        1: by apply expr_in_bij_subst.
+        1: by apply static_expr_subst.
+      * by tstep_s.
+      * revert select (Forall id _) => /Forall_zip_with_1 Hall.
+        move: (Hall ltac:(done)) => /Forall2_bij_val_inv_l[?[??]]; simplify_eq.
+        tstep_s. left. split! => ?. tend. split!; [solve_length|].
+        apply Hloop; [done|]. split!. 1: done. all: split!.
+        1: { apply expr_in_bij_subst_l; [|done|solve_length]. apply expr_in_bij_static. apply fd_static. }
+        apply static_expr_subst_l; [|solve_length]. apply static_expr_mono. apply fd_static.
+      * naive_solver.
+Qed.
+
+Lemma imp_heap_bij_imp_closed m σ:
+  trefines (MS (imp_closed (imp_heap_bij m)) (SMFilter, initial_imp_heap_bij_state m σ, ICStart))
+           (MS (imp_closed m) (SMFilter, σ, ICStart)).
+Proof.
+  apply tsim_implies_trefines => /= n.
+  unshelve apply: tsim_remember. { simpl. exact (λ _
+          '(σm1, (σf, σ1, (pp, ImpHeapBij bij hi)), σc1)
+          '(σm2, σ2, σc2),
+           σ1 = σ2 ∧ σc1 = σc2 ∧
+             ((σc1 = ICStart ∧ σf = SMFilter ∧ pp = PPOutside ∧ σm1 = σm2 ∧ σm2 = SMFilter ∧ bij = ∅) ∨
+              ( ((∃ e, σf = SMProgRecv e ∧ σm2 = SMProgRecv e) ∨ (σf = SMProg ∧ σm2 = SMProg)
+                 ) ∧ σm1 = SMProg ∧ σc1 = ICRunning ∧ pp = PPInside))
+                             ). }
+  { split!. } { done. }
+  move => {}n _ /= Hloop [[σm1 [[σf σ1] [pp [bij hi]]]] σc1] [[σm2 σ2] σc2] ?. destruct_all?; simplify_eq/=.
+  - tstep_i. apply steps_impl_step_end => ???. invert_all' @m_step; simplify_eq/=. split!.
+    tstep_s. eexists (Some (inr _)). split!. apply: steps_spec_step_end; [econs|] => ??. simplify_eq/=.
+    tstep_i. apply steps_impl_step_end => ???. invert_all @m_step. split!.
+    tstep_s. eexists (Some (inl _)). split!. apply: steps_spec_step_end; [econs|] => ??. simplify_eq/=.
+    tstep_i => ??; simplify_eq/=.
+    tstep_i. eexists ∅, (ValNum <$> vs), initial_heap_state. split!.
+    1: { apply Forall2_fmap. apply Forall_Forall2_diag. by apply Forall_true. }
+    apply: Hloop; [done|]. split!.
+  - tstep_both. apply steps_impl_step_end => κ ??. case_match => *; simplify_eq.
+    + tstep_s.  eexists (Some _). split; [done|]. apply: steps_spec_step_end; [done|] => ??. tend. split!; [done|].
+      apply: Hloop; [done|]. split!.
+    + tstep_s. eexists None. apply: steps_spec_step_end; [done|] => ??. tend. split!; [done|].
+      apply: Hloop; [done|]. split!.
+  - tstep_both. apply steps_impl_step_end => κ ??. tstep_s. eexists _. apply: steps_spec_step_end; [done|] => ??.
+    case_match; tend; (split!; [done|]). 2: { apply: Hloop; [done|]. split!. }
+    tstep_i => ? vs *. tstep_both => *.
+    apply steps_impl_step_end => ???. invert_all @m_step => ?; simplify_eq.
+    + destruct i as [? [? vs' |]]; simplify_eq/=.
+      tstep_s. eexists (Some _). split!.
+      apply: steps_spec_step_end; [econs|]=> /=??. destruct_all?; simplify_eq/=. tend.
+      split!.
+      tstep_both. apply steps_impl_step_end => ???. invert_all @m_step.
+      tstep_s. eexists (None). apply: steps_spec_step_end; [econs|]=> /=??. destruct_all?; simplify_eq/=. tend.
+      have ?: vs0 = ValNum <$> vs'0. {
+        revert select (m_step _ _ _ _) => _.
+        revert select (Forall2 _ _ _). elim: vs'0 vs0; csimpl => *; decompose_Forall_hyps => //.
+        match goal with |- ?x :: _ = _ => destruct x; simplify_eq/= => // end. naive_solver.
+      } subst.
+      split!; [done|].
+      tstep_i. apply steps_impl_step_end => ???. invert_all @m_step. split!.
+      tstep_s. eexists (Some (inr _)). split!. apply: steps_spec_step_end; [econs|] => /=? ->.
+      tstep_i. apply steps_impl_step_end => ???. invert_all @m_step. split!.
+      tstep_s. eexists (Some (inl _)). split!. apply: steps_spec_step_end; [econs|] => /=? ->.
+      tstep_i => ? <-.
+      tstep_i. eexists _, [ValNum _]. split!. 1: done. 1: done. 1: econs; [done|econs]. 1: done. 1: done.
+      apply: Hloop; [done|]. split!.
+    + destruct i as [? []]; simplify_eq/=.
+      tstep_s. eexists (Some _). split!.
+      apply: steps_spec_step_end; [econs|]=> /=??. destruct_all?; simplify_eq/=.
+      tstep_s. eexists None. apply: steps_spec_step_end; [econs|]=> /=??. destruct_all?; simplify_eq/=.
+      destruct vs as [|v ?]; decompose_Forall_hyps. destruct v => //; simplify_eq/=.
+      tend. split!.
+      tstep_i. apply: steps_impl_step_end => ???. invert_all @m_step. split!.
+      tstep_i. apply: steps_impl_step_end => ???. invert_all @m_step. split!.
+      tstep_s. eexists (Some (inr _)). split!.
+      apply: steps_spec_step_end; [econs|]=> /=? ->.
+      tstep_i. apply: steps_impl_step_end => ???. invert_all @m_step.
+Qed.
+
+Lemma imp_heap_bij_trefines_implies_ctx_refines fnsi fnss :
+  dom (gset _) fnsi = dom (gset _) fnss →
+  trefines (MS imp_module (initial_imp_state fnsi))
+           (MS (imp_heap_bij imp_module) (initial_imp_heap_bij_state imp_module (initial_imp_state fnss))) →
+  imp_ctx_refines fnsi fnss.
+Proof.
+  move => Hdom Href C. rewrite /imp_link map_difference_union_r (map_difference_union_r fnss).
+  etrans; [|apply imp_heap_bij_imp_closed].
+  apply mod_seq_map_trefines. { apply _. } { apply _. }
+  etrans. { apply imp_link_refines_prod. apply map_disjoint_difference_r'. }
+  etrans. { apply: imp_prod_trefines. 1: done. 1: apply imp_heap_bij_imp_refl. }
+  etrans. { apply imp_heap_bij_combine; apply _. }
+  apply: mod_prepost_trefines.
+  etrans. 2: { apply imp_prod_refines_link. apply map_disjoint_difference_r'. }
+  rewrite !dom_difference_L Hdom.
+  erewrite map_difference_eq_dom_L => //.
+  apply _.
+Qed.
